In polyScript, the polynomial operators have been overloaded. We are not sure whether this is a good idea or not.

src/real/polyScript.sml
@@ -15,7 +15,6 @@ app load ["numLib",
           "boolSimps",
           "arithSimps",
           "pairSimps",
-          "UnwindSimps",
           "Ho_rewrite",
           "jrhUtils",
           "limTheory",
@@ -83,17 +82,17 @@ val FORALL = LIST_CONJ (map SPEC_ALL (CONJUNCTS listTheory.EVERY_DEF));
 
 (* Basic extra theorems *)
 
-val FUN_EQ_THM = prove (``!f g.  (f = g) = (!x. f x = g x)``,
+val FUN_EQ_THM = prove (Term`!f g.  (f = g) = (!x. f x = g x)`,
   REPEAT GEN_TAC THEN EQ_TAC THENL
    [DISCH_THEN SUBST1_TAC THEN GEN_TAC THEN REFL_TAC,
     MATCH_ACCEPT_TAC EQ_EXT]);
 
 val RIGHT_IMP_EXISTS_THM = prove (
-  ``!P Q. P ==> (?x. Q x) = (?x. P ==> Q x)``,
+  Term`!P Q. P ==> (?x. Q x) = (?x. P ==> Q x)`,
   MESON_TAC []);
 
 val LEFT_IMP_EXISTS_THM = prove (
-  ``!P Q. (?x. P x) ==> Q = (!x. P x ==> Q)``,
+  Term`!P Q. (?x. P x) ==> Q = (!x. P x ==> Q)`,
   MESON_TAC []);
 
 (* Extra theorems needed about the naturals *)
@@ -101,46 +100,46 @@ val LEFT_IMP_EXISTS_THM = prove (
 val NOT_LE = arithmeticTheory.NOT_LESS_EQUAL;
 val SUC_INJ = prim_recTheory.INV_SUC_EQ
 
-val LT_SUC_LE = prove (``!m n. m < SUC n = m <= n``, ARITH_TAC);
+val LT_SUC_LE = prove (Term`!m n. m < SUC n = m <= n`, ARITH_TAC);
 
 val LT = prove(
-  ``(!m:num. m < 0 = F) /\ (!m n. m < SUC n = (m = n) \/ m < n)``,
+  Term`(!m:num. m < 0 = F) /\ (!m n. m < SUC n = (m = n) \/ m < n)`,
   ARITH_TAC);
 
 val LT_ADD_LCANCEL = prove (
-  ``!m n p:num. m + n < m + p = n < p``,
+  Term`!m n p:num. m + n < m + p = n < p`,
   ARITH_TAC);
 
 val LE_EXISTS = prove (
-  ``!m n:num. m <= n = (?d. n = m + d)``,
+  Term`!m n:num. m <= n = (?d. n = m + d)`,
   REPEAT (STRIP_TAC ORELSE EQ_TAC)
   THENL [
-    EXISTS_TAC ``n - m:num``,
+    EXISTS_TAC (Term`n - m:num`),
     ALL_TAC
   ]
   THEN POP_ASSUM (MP_TAC)
   THEN ARITH_TAC);
 
 val LE_SUC_LT = prove (
-  ``!m n. SUC m <= n = m < n``,
+  Term`!m n. SUC m <= n = m < n`,
   ARITH_TAC);
 
 val LT_CASES = prove (
-  ``!m n:num. m < n \/ n < m \/ (m = n)``,
+  Term`!m n:num. m < n \/ n < m \/ (m = n)`,
   ARITH_TAC);
 
-val LE_REFL = prove (``!n:num. n <= n``, ARITH_TAC);
+val LE_REFL = prove (Term`!n:num. n <= n`, ARITH_TAC);
 
 (* Extra theorems needed about sets *)
 
-val FINITE_SUBSET = prove (``!s t. FINITE t /\ s SUBSET t ==> FINITE s``,
+val FINITE_SUBSET = prove (Term`!s t. FINITE t /\ s SUBSET t ==> FINITE s`,
   MESON_TAC [SUBSET_FINITE]);
 
 val FINITE_RULES = prove (
-  ``FINITE {} /\ (!x s. FINITE s ==> FINITE (x INSERT s))``,
+  Term`FINITE {} /\ (!x s. FINITE s ==> FINITE (x INSERT s))`,
   MESON_TAC [FINITE_EMPTY, FINITE_INSERT]);
 
-val GSPEC_DEF = prove (``!f. GSPEC f = \v. ?z. f z = (v,T)``,
+val GSPEC_DEF = prove (Term`!f. GSPEC f = \v. ?z. f z = (v,T)`,
 GEN_TAC THEN CONV_TAC FUN_EQ_CONV THEN BETA_TAC THEN GEN_TAC
   THEN ONCE_REWRITE_TAC[BETA_RULE
         (ONCE_REWRITE_CONV[GSYM SPECIFICATION](Term`(\x. GSPEC f x) x`))]
@@ -153,36 +152,54 @@ GEN_TAC THEN CONV_TAC FUN_EQ_CONV THEN BETA_TAC THEN GEN_TAC
 (* ------------------------------------------------------------------------- *)
 
 val poly = new_recursive_definition list_Axiom "poly_def"
-  ``(poly [] x = &0) /\
-    (poly (CONS h t) x = h + x * poly t x)``;
+  (Term`(poly [] x = 0r) /\
+        (poly (h::t) x = h + x * poly t x)`);
 
 (* ------------------------------------------------------------------------- *)
-(* Arithmetic operations on polynomials.                                     *)
+(* Arithmetic operations on polynomials. Overloaded (not sure this is wise). *)
 (* ------------------------------------------------------------------------- *)
+
+val bool_not = Term`$~ : bool -> bool`;
+val natmult  = Term`$* : num -> num -> num`;
+val natplus  = Term`$+ : num -> num -> num`;
+
+val _ = allow_for_overloading_on ("~", Type`:'a -> 'a`);
+val _ = allow_for_overloading_on ("+", Type`:'a -> 'a -> 'a`);
+val _ = allow_for_overloading_on ("*", Type`:'a -> 'a -> 'a`);
+
+val _ = overload_on ("~", bool_not);
+val _ = overload_on ("+", natplus);
+val _ = overload_on ("*", natmult);
 
 val poly_add = new_recursive_definition list_Axiom "poly_add_def"
-  ``($++ [] l2 = l2) /\
-    ($++ (h::t) l2 = if (l2 = []) then h::t
-                    else CONS ((h:real) + HD l2) ($++ t (TL l2)))``;
-val _ = set_fixity "++" (Infixl 500);
+ (Term`(poly_add [] l2 = l2) /\
+       (poly_add (h::t) l2 = if (l2 = []) then h::t
+                             else  ((h:real) + HD l2)::poly_add t (TL l2))`);
+
+val _ = overload_on ("+", Term`poly_add`);
 
 val poly_cmul = new_recursive_definition list_Axiom "poly_cmul_def"
-  ``($## c [] = []) /\
-    ($## c (h::t) = (c:real * h) :: ($## c t))``;
-val _ = set_fixity "##" (Infixl 600);
+ (Term`($## c [] = []) /\
+       ($## c (h::t) = (c:real * h) :: ($## c t))`);
+val _ = set_fixity "##" (Infixl 600) ;
 
-val poly_neg = new_definition ("poly_neg_def", ``neg = $## (~(&1))``);
+val poly_neg = new_definition ("poly_neg_def", Term`poly_neg = $## (~(&1))`);
+
+val _ = overload_on ("~", Term`poly_neg`);
 
 val poly_mul = new_recursive_definition list_Axiom "poly_mul_def"
-  ``($** [] l2 = []) /\
-    ($** (h::t) l2 = if (t = []) then h ## l2
-                     else (h ## l2) ++ (&0 :: ($** t l2)))``;
-val _ = set_fixity "**" (Infixl 600);
+ (Term`(poly_mul [] l2     = []) /\
+       (poly_mul (h::t) l2 = if (t = []) then h ## l2
+                             else (h ## l2) + (0r :: poly_mul t l2))`);
 
-val poly_pexp = new_recursive_definition num_Axiom "poly_pexp_def"
-  ``($pexp p 0 = [&1]) /\
-    ($pexp p (SUC n) = p ** $pexp p n)``;
-val _ = set_fixity "pexp" (Infixr 700);
+val _ = overload_on ("*", Term`poly_mul`);
+
+val poly_exp = new_recursive_definition num_Axiom "poly_exp_def"
+ (Term`(poly_exp p 0       = [1r]) /\
+       (poly_exp p (SUC n) = poly_mul p (poly_exp p n))`);
+
+val _ = set_fixity "poly_exp" (Infixr 700) ;
+
 
 (* ------------------------------------------------------------------------- *)
 (* Differentiation of polynomials (needs an auxiliary function).             *)
@@ -190,44 +207,44 @@ val _ = set_fixity "pexp" (Infixr 700);
 
 val poly_diff_aux = new_recursive_definition list_Axiom
   "poly_diff_aux_def"
-  ``(poly_diff_aux n [] = []) /\
-    (poly_diff_aux n (h::t) = (&n * h) :: (poly_diff_aux (SUC n) t))``;
+   (Term`(poly_diff_aux n [] = []) /\
+         (poly_diff_aux n (h::t) = (&n * h) :: (poly_diff_aux (SUC n) t))`);
 
 val poly_diff = new_definition ("poly_diff_def",
-  ``diff l = (if (l = []) then [] else (poly_diff_aux 1 (TL l)))``);
+  Term`diff l = (if (l = []) then [] else (poly_diff_aux 1 (TL l)))`);
 
 (* ------------------------------------------------------------------------- *)
 (* Useful clausifications.                                                   *)
 (* ------------------------------------------------------------------------- *)
 
 val POLY_ADD_CLAUSES = store_thm("POLY_ADD_CLAUSES",
- ``([] ++ p2 = p2) /\
-   (p1 ++ [] = p1) /\
-   ((h1::t1) ++ (h2::t2) = CONS (h1 + h2) (t1 ++ t2))``,
+ Term`([] + p2 = p2) /\
+      (p1 + [] = p1) /\
+   ((h1::t1) + (h2::t2) =  (h1 + h2) :: (t1 + t2))`,
   REWRITE_TAC[poly_add, NOT_CONS_NIL, HD, TL] THEN
-  SPEC_TAC(``p1:real list``,``p1:real list``) THEN
+  SPEC_TAC(Term`p1:real list`,Term`p1:real list`) THEN
   LIST_INDUCT_TAC THEN ASM_REWRITE_TAC[poly_add]);
 
 val POLY_CMUL_CLAUSES = store_thm("POLY_CMUL_CLAUSES",
- ``(c ## [] = []) /\
-   (c ## (h::t) = (c * h) :: (c ## t))``,
+ Term`(c ## [] = []) /\
+      (c ## (h::t) = (c * h) :: (c ## t))`,
   REWRITE_TAC[poly_cmul]);
 
 val POLY_NEG_CLAUSES = store_thm("POLY_NEG_CLAUSES",
- ``(neg [] = []) /\
-   (neg (h::t) = ~h::neg t)``,
+ Term`(poly_neg [] = []) /\
+      (poly_neg (h::t) = ~h::poly_neg t)`,
   REWRITE_TAC[poly_neg, POLY_CMUL_CLAUSES, REAL_MUL_LNEG, REAL_MUL_LID]);
 
 val POLY_MUL_CLAUSES = store_thm("POLY_MUL_CLAUSES",
- ``([] ** p2 = []) /\
-   ([h1] ** p2 = h1 ## p2) /\
-   ((h1::k1::t1) ** p2 = (h1 ## p2) ++ (&0 :: ((k1::t1) ** p2)))``,
+ Term`([] * p2 = []) /\
+    ([h1] * p2 = h1 ## p2) /\
+   ((h1::k1::t1) * p2 = (h1 ## p2) + (&0 :: ((k1::t1) * p2)))`,
   REWRITE_TAC[poly_mul, NOT_CONS_NIL]);
 
 val POLY_DIFF_CLAUSES = store_thm("POLY_DIFF_CLAUSES",
- ``(diff [] = []) /\
+ Term`(diff [] = []) /\
    (diff [c] = []) /\
-   (diff (h::t) = poly_diff_aux 1 t)``,
+   (diff (h::t) = poly_diff_aux 1 t)`,
   REWRITE_TAC[poly_diff, NOT_CONS_NIL, HD, TL, poly_diff_aux]);
 
 (* ------------------------------------------------------------------------- *)
@@ -235,28 +252,28 @@ val POLY_DIFF_CLAUSES = store_thm("POLY_DIFF_CLAUSES",
 (* ------------------------------------------------------------------------- *)
 
 val POLY_ADD = store_thm("POLY_ADD",
- ``!p1 p2 x. poly (p1 ++ p2) x = poly p1 x + poly p2 x``,
+ Term`!p1 p2 x. poly (p1 + p2) x = poly p1 x + poly p2 x`,
   LIST_INDUCT_TAC THEN REWRITE_TAC[poly_add, poly, REAL_ADD_LID] THEN
   LIST_INDUCT_TAC THEN
   ASM_REWRITE_TAC[NOT_CONS_NIL, HD, TL, poly, REAL_ADD_RID] THEN
   REAL_ARITH_TAC);
 
 val POLY_CMUL = store_thm("POLY_CMUL",
- ``!p c x. poly (c ## p) x = c * poly p x``,
+ Term`!p c x. poly (c ## p) x = c * poly p x`,
   LIST_INDUCT_TAC THEN ASM_REWRITE_TAC[poly, poly_cmul] THEN
   REAL_ARITH_TAC);
 
 val POLY_NEG = store_thm("POLY_NEG",
- ``!p x. poly (neg p) x = ~(poly p x)``,
+ Term`!p x. poly (poly_neg p) x = ~(poly p x)`,
   REWRITE_TAC[poly_neg, POLY_CMUL] THEN
   REAL_ARITH_TAC);
 
 val POLY_MUL = store_thm("POLY_MUL",
- ``!x p1 p2. poly (p1 ** p2) x = poly p1 x * poly p2 x``,
+ Term`!x p1 p2. poly (p1 * p2) x = poly p1 x * poly p2 x`,
   GEN_TAC THEN LIST_INDUCT_TAC THEN
   REWRITE_TAC[poly_mul, poly, REAL_MUL_LZERO, POLY_CMUL, POLY_ADD] THEN
-  SPEC_TAC(``h:real``,``h:real``) THEN
-  SPEC_TAC(``t:real list``,``t:real list``) THEN
+  SPEC_TAC(Term`h:real`,Term`h:real`) THEN
+  SPEC_TAC(Term`t:real list`,Term`t:real list`) THEN
   LIST_INDUCT_TAC THEN
   REWRITE_TAC[poly_mul, POLY_CMUL, POLY_ADD, poly, POLY_CMUL,
     REAL_MUL_RZERO, REAL_ADD_RID, NOT_CONS_NIL] THEN
@@ -264,8 +281,8 @@ val POLY_MUL = store_thm("POLY_MUL",
   REAL_ARITH_TAC);
 
 val POLY_EXP = store_thm("POLY_EXP",
- ``!p n x. poly (p pexp n) x = (poly p x) pow n``,
-  GEN_TAC THEN INDUCT_TAC THEN ASM_REWRITE_TAC[poly_pexp, pow, POLY_MUL] THEN
+ Term`!p n (x:real). poly (p poly_exp n) x = (poly p x) pow n`,
+  GEN_TAC THEN INDUCT_TAC THEN ASM_REWRITE_TAC[poly_exp, pow, POLY_MUL] THEN
   REWRITE_TAC[poly] THEN REAL_ARITH_TAC);
 
 (* ------------------------------------------------------------------------- *)
@@ -273,35 +290,35 @@ val POLY_EXP = store_thm("POLY_EXP",
 (* ------------------------------------------------------------------------- *)
 
 val POLY_DIFF_LEMMA = store_thm("POLY_DIFF_LEMMA",
- ``!l n x. ((\x. (x pow (SUC n)) * poly l x) diffl
-                   ((x pow n) * poly (poly_diff_aux (SUC n) l) x))(x)``,
+ (Term`!l n x. ((\x. (x pow (SUC n)) * poly l x) diffl
+                   ((x pow n) * poly (poly_diff_aux (SUC n) l) x))(x)`),
   LIST_INDUCT_TAC THEN
   REWRITE_TAC[poly, poly_diff_aux, REAL_MUL_RZERO, DIFF_CONST] THEN
-  MAP_EVERY X_GEN_TAC [``n:num``, ``x:real``] THEN
+  MAP_EVERY X_GEN_TAC [(Term`n:num`), (Term`x:real`)] THEN
   REWRITE_TAC[REAL_LDISTRIB, REAL_MUL_ASSOC] THEN
   ONCE_REWRITE_TAC[GSYM(ONCE_REWRITE_RULE[REAL_MUL_SYM] (CONJUNCT2 pow))] THEN
-  POP_ASSUM(MP_TAC o SPECL [``SUC n``, ``x:real``]) THEN
-  SUBGOAL_THEN ``(((\x. (x pow (SUC n)) * h)) diffl
-                        ((x pow n) * &(SUC n) * h))(x)``
+  POP_ASSUM(MP_TAC o SPECL [(Term`SUC n`), (Term`x:real`)]) THEN
+  SUBGOAL_THEN ((Term`(((\x. (x pow (SUC n)) * h)) diffl
+                        ((x pow n) * &(SUC n) * h))(x)`))
   (fn th => DISCH_THEN(MP_TAC o CONJ th)) THENL
    [REWRITE_TAC[REAL_MUL_ASSOC] THEN ONCE_REWRITE_TAC[REAL_MUL_SYM] THEN
-    MP_TAC(SPEC ``\x. x pow (SUC n)`` DIFF_CMUL) THEN BETA_TAC THEN
+    MP_TAC(SPEC ((Term`\x. x pow (SUC n)`)) DIFF_CMUL) THEN BETA_TAC THEN
     DISCH_THEN MATCH_MP_TAC THEN
-    MP_TAC(SPEC ``SUC n`` DIFF_POW) THEN REWRITE_TAC[SUC_SUB1] THEN
+    MP_TAC(SPEC ((Term`SUC n`)) DIFF_POW) THEN REWRITE_TAC[SUC_SUB1] THEN
     DISCH_THEN(MATCH_ACCEPT_TAC o ONCE_REWRITE_RULE[REAL_MUL_SYM]),
     DISCH_THEN(MP_TAC o MATCH_MP DIFF_ADD) THEN BETA_TAC THEN
     REWRITE_TAC[REAL_MUL_ASSOC]]);
 
 val POLY_DIFF = store_thm("POLY_DIFF",
- ``!l x. ((\x. poly l x) diffl (poly (diff l) x))(x)``,
+ (Term`!l x. ((\x. poly l x) diffl (poly (diff l) x))(x)`),
   LIST_INDUCT_TAC THEN REWRITE_TAC[POLY_DIFF_CLAUSES] THEN
-  ONCE_REWRITE_TAC[SYM(ETA_CONV ``\x. poly l x``)] THEN
+  ONCE_REWRITE_TAC[SYM(ETA_CONV (Term`\x. poly l x`))] THEN
   REWRITE_TAC[poly, DIFF_CONST] THEN
-  MAP_EVERY X_GEN_TAC [``x:real``] THEN
-  MP_TAC(SPECL [``t:real list``, ``0:num``, ``x:real``] POLY_DIFF_LEMMA) THEN
+  MAP_EVERY X_GEN_TAC [(Term`x:real`)] THEN
+  MP_TAC(SPECL [(Term`t:real list`), (Term`0:num`), (Term`x:real`)] POLY_DIFF_LEMMA) THEN
   REWRITE_TAC[SYM ONE] THEN REWRITE_TAC[pow, REAL_MUL_LID] THEN
   REWRITE_TAC[POW_1] THEN
-  DISCH_THEN(MP_TAC o CONJ (SPECL [``h:real``, ``x:real``] DIFF_CONST)) THEN
+  DISCH_THEN(MP_TAC o CONJ (SPECL [(Term`h:real`), (Term`x:real`)] DIFF_CONST)) THEN
   DISCH_THEN(MP_TAC o MATCH_MP DIFF_ADD) THEN BETA_TAC THEN
   REWRITE_TAC[REAL_ADD_LID]);
 
@@ -310,53 +327,53 @@ val POLY_DIFF = store_thm("POLY_DIFF",
 (* ------------------------------------------------------------------------- *)
 
 val POLY_DIFFERENTIABLE = store_thm("POLY_DIFFERENTIABLE",
- ``!l x. (\x. poly l x) differentiable x``,
+ (Term`!l x. (\x. poly l x) differentiable x`),
   REPEAT GEN_TAC THEN REWRITE_TAC[differentiable] THEN
-  EXISTS_TAC ``poly (diff l) x`` THEN
+  EXISTS_TAC (Term`poly (diff l) x`) THEN
   REWRITE_TAC[POLY_DIFF]);
 
 val POLY_CONT = store_thm("POLY_CONT",
- ``!l x. (\x. poly l x) contl x``,
+ (Term`!l x. (\x. poly l x) contl x`),
   REPEAT GEN_TAC THEN MATCH_MP_TAC DIFF_CONT THEN
-  EXISTS_TAC ``poly (diff l) x`` THEN
+  EXISTS_TAC (Term`poly (diff l) x`) THEN
   MATCH_ACCEPT_TAC POLY_DIFF);
 
 val POLY_IVT_POS = store_thm("POLY_IVT_POS",
- ``!p a b. a < b /\ poly p a < &0 /\ poly p b > &0
-           ==> ?x. a < x /\ x < b /\ (poly p x = &0)``,
+ (Term`!p a b. a < b /\ poly p a < &0 /\ poly p b > &0
+           ==> ?x. a < x /\ x < b /\ (poly p x = &0)`),
   REWRITE_TAC[real_gt] THEN REPEAT STRIP_TAC THEN
-  MP_TAC(SPECL [``\x. poly p x``, ``a:real``, ``b:real``, ``&0``] IVT) THEN
+  MP_TAC(SPECL [(Term`\x. poly p x`), (Term`a:real`), (Term`b:real`), (Term`&0`)] IVT) THEN
   SIMP_TAC bool_ss [POLY_CONT] THEN
   EVERY_ASSUM(fn th => REWRITE_TAC[MATCH_MP REAL_LT_IMP_LE th]) THEN
-  DISCH_THEN(X_CHOOSE_THEN ``x:real`` STRIP_ASSUME_TAC) THEN
-  EXISTS_TAC ``x:real`` THEN ASM_REWRITE_TAC[REAL_LT_LE] THEN
+  DISCH_THEN(X_CHOOSE_THEN (Term`x:real`) STRIP_ASSUME_TAC) THEN
+  EXISTS_TAC (Term`x:real`) THEN ASM_REWRITE_TAC[REAL_LT_LE] THEN
   CONJ_TAC THEN DISCH_THEN SUBST_ALL_TAC THEN
   FIRST_ASSUM SUBST_ALL_TAC THEN
   RULE_ASSUM_TAC(REWRITE_RULE[REAL_LT_REFL]) THEN
   FIRST_ASSUM CONTR_TAC);
 
 val POLY_IVT_NEG = store_thm("POLY_IVT_NEG",
- ``!p a b. a < b /\ poly p a > &0 /\ poly p b < &0
-           ==> ?x. a < x /\ x < b /\ (poly p x = &0)``,
-  REPEAT STRIP_TAC THEN MP_TAC(SPEC ``neg p`` POLY_IVT_POS) THEN
+ (Term`!p a b. a < b /\ poly p a > &0 /\ poly p b < &0
+           ==> ?x. a < x /\ x < b /\ (poly p x = &0)`),
+  REPEAT STRIP_TAC THEN MP_TAC(SPEC (Term`poly_neg p`) POLY_IVT_POS) THEN
   REWRITE_TAC[POLY_NEG,
-              REAL_ARITH ``(~x < &0 = x > &0) /\ (~x > &0 = x < &0)``] THEN
-  DISCH_THEN(MP_TAC o SPECL [``a:real``, ``b:real``]) THEN
-  ASM_REWRITE_TAC[REAL_ARITH ``(~x = &0) = (x = &0)``]);
+              REAL_ARITH (Term`(~x < &0 = x > &0) /\ (~x > &0 = x < &0)`)] THEN
+  DISCH_THEN(MP_TAC o SPECL [(Term`a:real`), (Term`b:real`)]) THEN
+  ASM_REWRITE_TAC[REAL_ARITH (Term`(~x = &0) = (x = &0)`)]);
 
 val POLY_MVT = store_thm("POLY_MVT",
- ``!p a b. a < b ==>
+ (Term`!p a b. a < b ==>
            ?x. a < x /\ x < b /\
-              (poly p b - poly p a = (b - a) * poly (diff p) x)``,
+              (poly p b - poly p a = (b - a) * poly (diff p) x)`),
   REPEAT STRIP_TAC THEN
-  MP_TAC(SPECL [``poly p``, ``a:real``, ``b:real``] MVT) THEN
+  MP_TAC(SPECL [(Term`poly p`), (Term`a:real`), (Term`b:real`)] MVT) THEN
   ASM_REWRITE_TAC[CONV_RULE(DEPTH_CONV ETA_CONV) (SPEC_ALL POLY_CONT),
     CONV_RULE(DEPTH_CONV ETA_CONV) (SPEC_ALL POLY_DIFFERENTIABLE)] THEN
-  DISCH_THEN(X_CHOOSE_THEN ``l:real`` MP_TAC) THEN
-  DISCH_THEN(X_CHOOSE_THEN ``x:real`` STRIP_ASSUME_TAC) THEN
-  EXISTS_TAC ``x:real`` THEN ASM_REWRITE_TAC[] THEN
+  DISCH_THEN(X_CHOOSE_THEN (Term`l:real`) MP_TAC) THEN
+  DISCH_THEN(X_CHOOSE_THEN (Term`x:real`) STRIP_ASSUME_TAC) THEN
+  EXISTS_TAC (Term`x:real`) THEN ASM_REWRITE_TAC[] THEN
   AP_TERM_TAC THEN MATCH_MP_TAC DIFF_UNIQ THEN
-  EXISTS_TAC ``poly p`` THEN EXISTS_TAC ``x:real`` THEN
+  EXISTS_TAC (Term`poly p`) THEN EXISTS_TAC (Term`x:real`) THEN
   ASM_REWRITE_TAC[CONV_RULE(DEPTH_CONV ETA_CONV) (SPEC_ALL POLY_DIFF)]);
 
 (* ------------------------------------------------------------------------- *)
@@ -364,17 +381,17 @@ val POLY_MVT = store_thm("POLY_MVT",
 (* ------------------------------------------------------------------------- *)
 
 val POLY_ADD_RZERO = store_thm("POLY_ADD_RZERO",
- ``!p. poly (p ++ []) = poly p``,
+ (Term`!p. poly (p + []) = poly p`),
   REWRITE_TAC[FUN_EQ_THM, POLY_ADD, poly, REAL_ADD_RID]);
 
 val POLY_MUL_ASSOC = store_thm("POLY_MUL_ASSOC",
- ``!p q r. poly (p ** (q ** r)) = poly ((p ** q) ** r)``,
+ (Term`!p q r. poly (p * (q * r)) = poly ((p * q) * r)`),
   REWRITE_TAC[FUN_EQ_THM, POLY_MUL, REAL_MUL_ASSOC]);
 
 val POLY_EXP_ADD = store_thm("POLY_EXP_ADD",
- ``!d n p. poly(p pexp (n + d)) = poly(p pexp n ** p pexp d)``,
+ (Term`!d n p. poly(p poly_exp (n + d)) = poly(p poly_exp n * p poly_exp d)`),
   REWRITE_TAC[FUN_EQ_THM, POLY_MUL] THEN
-  INDUCT_TAC THEN ASM_REWRITE_TAC[POLY_MUL, ADD_CLAUSES, poly_pexp, poly] THEN
+  INDUCT_TAC THEN ASM_REWRITE_TAC[POLY_MUL, ADD_CLAUSES, poly_exp, poly] THEN
   REAL_ARITH_TAC);
 
 (* ------------------------------------------------------------------------- *)
@@ -382,25 +399,25 @@ val POLY_EXP_ADD = store_thm("POLY_EXP_ADD",
 (* ------------------------------------------------------------------------- *)
 
 val POLY_DIFF_AUX_ADD = store_thm("POLY_DIFF_AUX_ADD",
-``!p1 p2 n. poly (poly_diff_aux n (p1 ++ p2)) =
-             poly (poly_diff_aux n p1 ++ poly_diff_aux n p2)``,
+(Term`!p1 p2 n. poly (poly_diff_aux n (p1 + p2)) =
+             poly (poly_diff_aux n p1 + poly_diff_aux n p2)`),
   REPEAT(LIST_INDUCT_TAC THEN REWRITE_TAC[poly_diff_aux, poly_add]) THEN
   ASM_REWRITE_TAC[poly_diff_aux, FUN_EQ_THM, poly, NOT_CONS_NIL, HD, TL] THEN
   REAL_ARITH_TAC);
 
 val POLY_DIFF_AUX_CMUL = store_thm("POLY_DIFF_AUX_CMUL",
- ``!p c n. poly (poly_diff_aux n (c ## p)) =
-           poly (c ## poly_diff_aux n p)``,
+ (Term`!p c n. poly (poly_diff_aux n (c ## p)) =
+           poly (c ## poly_diff_aux n p)`),
   LIST_INDUCT_TAC THEN
   ASM_SIMP_TAC real_ss [FUN_EQ_THM, poly, poly_diff_aux, poly_cmul]);
 
 val POLY_DIFF_AUX_NEG = store_thm("POLY_DIFF_AUX_NEG",
- ``!p n.  poly (poly_diff_aux n (neg p)) =
-          poly (neg (poly_diff_aux n p))``,
+ (Term`!p n.  poly (poly_diff_aux n (poly_neg p)) =
+          poly (poly_neg (poly_diff_aux n p))`),
   REWRITE_TAC[poly_neg, POLY_DIFF_AUX_CMUL]);
 
 val POLY_DIFF_AUX_MUL_LEMMA = store_thm("POLY_DIFF_AUX_MUL_LEMMA",
- ``!p n. poly (poly_diff_aux (SUC n) p) = poly (poly_diff_aux n p ++ p)``,
+ (Term`!p n. poly (poly_diff_aux (SUC n) p) = poly (poly_diff_aux n p + p)`),
   LIST_INDUCT_TAC THEN REWRITE_TAC[poly_diff_aux, poly_add, NOT_CONS_NIL] THEN
   ASM_REWRITE_TAC[HD, TL, poly, FUN_EQ_THM] THEN
   REWRITE_TAC[GSYM REAL_OF_NUM_SUC, REAL_ADD_RDISTRIB, REAL_MUL_LID]);
@@ -410,24 +427,24 @@ val POLY_DIFF_AUX_MUL_LEMMA = store_thm("POLY_DIFF_AUX_MUL_LEMMA",
 (* ------------------------------------------------------------------------- *)
 
 val POLY_DIFF_ADD = store_thm("POLY_DIFF_ADD",
- ``!p1 p2. poly (diff (p1 ++ p2)) =
-           poly (diff p1  ++ diff p2)``,
+ (Term`!p1 p2. poly (diff (p1 + p2)) =
+           poly (diff p1  + diff p2)`),
   REPEAT LIST_INDUCT_TAC THEN
   REWRITE_TAC[poly_add, poly_diff, NOT_CONS_NIL, POLY_ADD_RZERO] THEN
   ASM_REWRITE_TAC[HD, TL, POLY_DIFF_AUX_ADD]);
 
 val POLY_DIFF_CMUL = store_thm("POLY_DIFF_CMUL",
- ``!p c. poly (diff (c ## p)) = poly (c ## diff p)``,
+ (Term`!p c. poly (diff (c ## p)) = poly (c ## diff p)`),
   LIST_INDUCT_TAC THEN REWRITE_TAC[poly_diff, poly_cmul] THEN
   REWRITE_TAC[NOT_CONS_NIL, HD, TL, POLY_DIFF_AUX_CMUL]);
 
 val POLY_DIFF_NEG = store_thm("POLY_DIFF_NEG",
- ``!p. poly (diff (neg p)) = poly (neg (diff p))``,
+ (Term`!p. poly (diff (poly_neg p)) = poly (poly_neg (diff p))`),
   REWRITE_TAC[poly_neg, POLY_DIFF_CMUL]);
 
 val POLY_DIFF_MUL_LEMMA = store_thm("POLY_DIFF_MUL_LEMMA",
- ``!t h. poly (diff (CONS h t)) =
-         poly (CONS (&0) (diff t) ++ t)``,
+ (Term`!t h. poly (diff (CONS h t)) =
+         poly (CONS (&0) (diff t) + t)`),
   REWRITE_TAC[poly_diff, NOT_CONS_NIL] THEN
   LIST_INDUCT_TAC THEN REWRITE_TAC[poly_diff_aux, NOT_CONS_NIL, HD, TL] THENL
    [REWRITE_TAC[FUN_EQ_THM, poly, poly_add, REAL_MUL_RZERO, REAL_ADD_LID],
@@ -435,8 +452,8 @@ val POLY_DIFF_MUL_LEMMA = store_thm("POLY_DIFF_MUL_LEMMA",
     REAL_ARITH_TAC]);
 
 val POLY_DIFF_MUL = store_thm("POLY_DIFF_MUL",
- ``!p1 p2. poly (diff (p1 ** p2)) =
-           poly (p1 ** diff p2 ++ diff p1 ** p2)``,
+ (Term`!p1 p2. poly (diff (p1 * p2)) =
+           poly (p1 * diff p2 + diff p1 * p2)`),
   LIST_INDUCT_TAC THEN REWRITE_TAC[poly_mul] THENL
    [REWRITE_TAC[poly_diff, poly_add, poly_mul], ALL_TAC] THEN
   GEN_TAC THEN COND_CASES_TAC THEN ASM_REWRITE_TAC[] THENL
@@ -449,22 +466,22 @@ val POLY_DIFF_MUL = store_thm("POLY_DIFF_MUL",
   REAL_ARITH_TAC);
 
 val POLY_DIFF_EXP = store_thm("POLY_DIFF_EXP",
- ``!p n. poly (diff (p pexp (SUC n))) =
-         poly (&(SUC n) ## (p pexp n) ** diff p)``,
-  GEN_TAC THEN INDUCT_TAC THEN ONCE_REWRITE_TAC[poly_pexp] THENL
-   [REWRITE_TAC[poly_pexp, POLY_DIFF_MUL] THEN
+ (Term`!p n. poly (diff (p poly_exp (SUC n))) =
+         poly (&(SUC n) ## (p poly_exp n) * diff p)`),
+  GEN_TAC THEN INDUCT_TAC THEN ONCE_REWRITE_TAC[poly_exp] THENL
+   [REWRITE_TAC[poly_exp, POLY_DIFF_MUL] THEN
     REWRITE_TAC[FUN_EQ_THM, POLY_MUL, POLY_ADD, POLY_CMUL] THEN
     REWRITE_TAC[poly, POLY_DIFF_CLAUSES, ADD1, ADD_CLAUSES] THEN
     REAL_ARITH_TAC,
     REWRITE_TAC[POLY_DIFF_MUL] THEN
     ASM_REWRITE_TAC[POLY_MUL, POLY_ADD, FUN_EQ_THM, POLY_CMUL] THEN
-    REWRITE_TAC[poly_pexp, POLY_MUL] THEN
+    REWRITE_TAC[poly_exp, POLY_MUL] THEN
     REWRITE_TAC[ADD1, GSYM REAL_OF_NUM_ADD] THEN
     REAL_ARITH_TAC]);
 
 val POLY_DIFF_EXP_PRIME = store_thm("POLY_DIFF_EXP_PRIME",
- ``!n a. poly (diff ([~a; &1] pexp (SUC n))) =
-         poly (&(SUC n) ## ([~a; &1] pexp n))``,
+ (Term`!n a. poly (diff ([~a; &1] poly_exp (SUC n))) =
+         poly (&(SUC n) ## ([~a; &1] poly_exp n))`),
   REPEAT GEN_TAC THEN SIMP_TAC real_ss [POLY_DIFF_EXP] THEN
   SIMP_TAC real_ss [FUN_EQ_THM, POLY_CMUL, POLY_MUL] THEN
   SIMP_TAC real_ss [poly_diff, poly_diff_aux, TL, NOT_CONS_NIL] THEN
@@ -475,54 +492,56 @@ val POLY_DIFF_EXP_PRIME = store_thm("POLY_DIFF_EXP_PRIME",
 (* ------------------------------------------------------------------------- *)
 
 val POLY_LINEAR_REM = store_thm("POLY_LINEAR_REM",
- ``!t h. ?q r. CONS h t = [r] ++ [~a; &1] ** q``,
+ (Term`!t h. ?q r. h::t = [r] + [~a; &1] * q`),
   LIST_INDUCT_TAC THEN REWRITE_TAC[] THENL
-   [GEN_TAC THEN EXISTS_TAC ``[]:real list`` THEN
-    EXISTS_TAC ``h:real`` THEN
+   [GEN_TAC THEN EXISTS_TAC (Term`[]:real list`) THEN
+    EXISTS_TAC (Term`h:real`) THEN
     REWRITE_TAC[poly_add, poly_mul, poly_cmul, NOT_CONS_NIL] THEN
     REWRITE_TAC[HD, TL, REAL_ADD_RID],
-    X_GEN_TAC ``k:real`` THEN POP_ASSUM(STRIP_ASSUME_TAC o SPEC ``h:real``) THEN
-    EXISTS_TAC ``CONS (r:real) q`` THEN EXISTS_TAC ``r * a + k`` THEN
+    X_GEN_TAC (Term`k:real`) THEN 
+    POP_ASSUM(STRIP_ASSUME_TAC o SPEC (Term`h:real`)) THEN
+    EXISTS_TAC (Term`CONS (r:real) q`) THEN 
+    EXISTS_TAC (Term`r * a + k:real`) THEN
     ASM_REWRITE_TAC[POLY_ADD_CLAUSES, POLY_MUL_CLAUSES, poly_cmul] THEN
     REWRITE_TAC[CONS_11] THEN CONJ_TAC THENL
      [REAL_ARITH_TAC, ALL_TAC] THEN
-    SPEC_TAC(``q:real list``,``q:real list``) THEN
+    SPEC_TAC((Term`q:real list`),(Term`q:real list`)) THEN
     LIST_INDUCT_TAC THEN
     REWRITE_TAC[POLY_ADD_CLAUSES, POLY_MUL_CLAUSES, poly_cmul] THEN
     REWRITE_TAC[REAL_ADD_RID, REAL_MUL_LID] THEN
     SIMP_TAC real_ss []]);
 
 val POLY_LINEAR_DIVIDES = store_thm("POLY_LINEAR_DIVIDES",
- ``!a p. (poly p a = &0) = (p = []) \/ ?q. p = [~a; &1] ** q``,
+ (Term`!a p. (poly p a = &0) = (p = []) \/ ?q. p = [~a; &1] * q`),
   GEN_TAC THEN LIST_INDUCT_TAC THENL
    [REWRITE_TAC[poly], ALL_TAC] THEN
   EQ_TAC THEN STRIP_TAC THENL
    [DISJ2_TAC THEN STRIP_ASSUME_TAC(SPEC_ALL POLY_LINEAR_REM) THEN
-    EXISTS_TAC ``q:real list`` THEN ASM_REWRITE_TAC[] THEN
-    SUBGOAL_THEN ``r = &0`` SUBST_ALL_TAC THENL
-     [UNDISCH_TAC ``poly (CONS h t) a = &0`` THEN
+    EXISTS_TAC (Term`q:real list`) THEN ASM_REWRITE_TAC[] THEN
+    SUBGOAL_THEN (Term`r = &0`) SUBST_ALL_TAC THENL
+     [UNDISCH_TAC (Term`poly (CONS h t) a = &0`) THEN
       ASM_REWRITE_TAC[] THEN REWRITE_TAC[POLY_ADD, POLY_MUL] THEN
       REWRITE_TAC[poly, REAL_MUL_RZERO, REAL_ADD_RID, REAL_MUL_RID] THEN
-      REWRITE_TAC[REAL_ARITH ``~a + a = &0``] THEN REAL_ARITH_TAC,
+      REWRITE_TAC[REAL_ARITH (Term`~a + a = &0`)] THEN REAL_ARITH_TAC,
       REWRITE_TAC[poly_mul] THEN REWRITE_TAC[NOT_CONS_NIL] THEN
-      SPEC_TAC(``q:real list``,``q:real list``) THEN LIST_INDUCT_TAC THENL
+      SPEC_TAC((Term`q:real list`),(Term`q:real list`)) THEN LIST_INDUCT_TAC THENL
        [REWRITE_TAC[poly_cmul, poly_add, NOT_CONS_NIL, HD, TL, REAL_ADD_LID],
         REWRITE_TAC[poly_cmul, poly_add, NOT_CONS_NIL, HD, TL, REAL_ADD_LID]]],
     ASM_REWRITE_TAC[] THEN REWRITE_TAC[poly],
     ASM_REWRITE_TAC[] THEN REWRITE_TAC[poly] THEN
     REWRITE_TAC[POLY_MUL] THEN REWRITE_TAC[poly] THEN
     REWRITE_TAC[poly, REAL_MUL_RZERO, REAL_ADD_RID, REAL_MUL_RID] THEN
-    REWRITE_TAC[REAL_ARITH ``~a + a = &0``] THEN REAL_ARITH_TAC]);
+    REWRITE_TAC[REAL_ARITH (Term`~a + a = &0`)] THEN REAL_ARITH_TAC]);
 
 (* ------------------------------------------------------------------------- *)
 (* Thanks to the finesse of the above, we can use length rather than degree. *)
 (* ------------------------------------------------------------------------- *)
 
 val POLY_LENGTH_MUL = store_thm("POLY_LENGTH_MUL",
- ``!q. LENGTH([~a; &1] ** q) = SUC(LENGTH q)``,
+ (Term`!q. LENGTH([~a; &1] * q) = SUC(LENGTH q)`),
   let
     val lemma = prove
-   (``!p h k a. LENGTH (k ## p ++ CONS h (a ## p)) = SUC(LENGTH p)``,
+   ((Term`!p h k a. LENGTH (k ## p + CONS h (a ## p)) = SUC(LENGTH p)`),
     LIST_INDUCT_TAC THEN
     ASM_REWRITE_TAC[poly_cmul, POLY_ADD_CLAUSES, LENGTH])
   in
@@ -534,68 +553,68 @@ val POLY_LENGTH_MUL = store_thm("POLY_LENGTH_MUL",
 (* ------------------------------------------------------------------------- *)
 
 val POLY_ROOTS_INDEX_LEMMA = store_thm("POLY_ROOTS_INDEX_LEMMA",
- ``!n. !p. ~(poly p = poly []) /\ (LENGTH p = n)
-           ==> ?i. !x. (poly p (x) = &0) ==> ?m. m <= n /\ (x = i m)``,
+ (Term`!n. !p. ~(poly p = poly []) /\ (LENGTH p = n)
+           ==> ?i. !x. (poly p (x) = &0) ==> ?m. m <= n /\ (x = i m)`),
   INDUCT_TAC THENL
    [SIMP_TAC real_ss [LENGTH_NIL],
-    REPEAT STRIP_TAC THEN ASM_CASES_TAC ``?a. poly p a = &0`` THENL
-     [UNDISCH_TAC ``?a. poly p a = &0`` THEN DISCH_THEN(CHOOSE_THEN MP_TAC) THEN
+    REPEAT STRIP_TAC THEN ASM_CASES_TAC (Term`?a. poly p a = &0`) THENL
+     [UNDISCH_TAC (Term`?a. poly p a = &0`) THEN DISCH_THEN(CHOOSE_THEN MP_TAC) THEN
       GEN_REWRITE_TAC LAND_CONV [POLY_LINEAR_DIVIDES] THEN
       DISCH_THEN(DISJ_CASES_THEN MP_TAC) THENL [ASM_MESON_TAC[], ALL_TAC] THEN
-      DISCH_THEN(X_CHOOSE_THEN ``q:real list`` SUBST_ALL_TAC) THEN
+      DISCH_THEN(X_CHOOSE_THEN (Term`q:real list`) SUBST_ALL_TAC) THEN
       FIRST_ASSUM(UNDISCH_TAC o assert is_forall o concl) THEN
-      UNDISCH_TAC ``~(poly ([~a; &1] ** q) = poly [])`` THEN
+      UNDISCH_TAC (Term`~(poly ([~a; &1] * q) = poly [])`) THEN
       POP_ASSUM MP_TAC THEN REWRITE_TAC[POLY_LENGTH_MUL, SUC_INJ] THEN
-      DISCH_TAC THEN ASM_CASES_TAC ``poly q = poly []`` THENL
+      DISCH_TAC THEN ASM_CASES_TAC (Term`poly q = poly []`) THENL
        [ASM_REWRITE_TAC[POLY_MUL, poly, REAL_MUL_RZERO, FUN_EQ_THM],
         DISCH_THEN(K ALL_TAC)] THEN
-      DISCH_THEN(MP_TAC o SPEC ``q:real list``) THEN ASM_REWRITE_TAC[] THEN
-      DISCH_THEN(X_CHOOSE_TAC ``i:num->real``) THEN
-      EXISTS_TAC ``\m. if m = SUC n then (a:real) else i m`` THEN
+      DISCH_THEN(MP_TAC o SPEC (Term`q:real list`)) THEN ASM_REWRITE_TAC[] THEN
+      DISCH_THEN(X_CHOOSE_TAC (Term`i:num->real`)) THEN
+      EXISTS_TAC (Term`\m. if m = SUC n then (a:real) else i m`) THEN
       REWRITE_TAC[POLY_MUL, LE, REAL_ENTIRE] THEN
-      X_GEN_TAC ``x:real`` THEN DISCH_THEN(DISJ_CASES_THEN MP_TAC) THENL
-       [DISCH_THEN(fn th => EXISTS_TAC ``SUC n`` THEN MP_TAC th) THEN
+      X_GEN_TAC (Term`x:real`) THEN DISCH_THEN(DISJ_CASES_THEN MP_TAC) THENL
+       [DISCH_THEN(fn th => EXISTS_TAC (Term`SUC n`) THEN MP_TAC th) THEN
         SIMP_TAC real_ss [] THEN REWRITE_TAC[poly] THEN REAL_ARITH_TAC,
         DISCH_THEN(ANTE_RES_THEN MP_TAC) THEN
-        DISCH_THEN(X_CHOOSE_THEN ``m:num`` STRIP_ASSUME_TAC) THEN
-        EXISTS_TAC ``m:num`` THEN ASM_SIMP_TAC real_ss [] THEN
+        DISCH_THEN(X_CHOOSE_THEN (Term`m:num`) STRIP_ASSUME_TAC) THEN
+        EXISTS_TAC (Term`m:num`) THEN ASM_SIMP_TAC real_ss [] THEN
         COND_CASES_TAC THEN ASM_REWRITE_TAC[] THEN
-        UNDISCH_TAC ``m:num <= n`` THEN ASM_SIMP_TAC real_ss []],
-      UNDISCH_TAC ``~(?a. poly p a = &0)`` THEN
+        UNDISCH_TAC (Term`m:num <= n`) THEN ASM_SIMP_TAC real_ss []],
+      UNDISCH_TAC (Term`~(?a. poly p a = &0)`) THEN
       REWRITE_TAC[NOT_EXISTS_THM] THEN DISCH_TAC
       THEN ASM_SIMP_TAC bool_ss []]]);
 
 val POLY_ROOTS_INDEX_LENGTH = store_thm("POLY_ROOTS_INDEX_LENGTH",
- ``!p. ~(poly p = poly [])
-       ==> ?i. !x. (poly p(x) = &0) ==> ?n. n <= LENGTH p /\ (x = i n)``,
+ (Term`!p. ~(poly p = poly [])
+       ==> ?i. !x. (poly p(x) = &0) ==> ?n. n <= LENGTH p /\ (x = i n)`),
   MESON_TAC[POLY_ROOTS_INDEX_LEMMA]);
 
 val POLY_ROOTS_FINITE_LEMMA = store_thm("POLY_ROOTS_FINITE_LEMMA",
- ``!p. ~(poly p = poly [])
-       ==> ?N i. !x. (poly p(x) = &0) ==> ?n:num. n < N /\ (x = i n)``,
+ (Term`!p. ~(poly p = poly [])
+       ==> ?N i. !x. (poly p(x) = &0) ==> ?n:num. n < N /\ (x = i n)`),
   MESON_TAC[POLY_ROOTS_INDEX_LENGTH, LT_SUC_LE]);
 
 val FINITE_LEMMA = store_thm("FINITE_LEMMA",
- ``!i N P. (!x. P x ==> ?n:num. n < N /\ (x = i n))
-           ==> ?a. !x. P x ==> x < a``,
+ (Term`!i N P. (!x. P x ==> ?n:num. n < N /\ (x = i n))
+           ==> ?a. !x. P x ==> x < a`),
   GEN_TAC THEN ONCE_REWRITE_TAC[RIGHT_IMP_EXISTS_THM] THEN INDUCT_TAC THENL
    [REWRITE_TAC[LT] THEN MESON_TAC[], ALL_TAC] THEN
-  X_GEN_TAC ``P:real->bool`` THEN
-  POP_ASSUM(MP_TAC o SPEC ``\z. P z /\ ~(z = (i:num->real) N)``) THEN
-  DISCH_THEN(X_CHOOSE_TAC ``a:real``) THEN
-  EXISTS_TAC ``abs(a) + abs(i(N:num)) + &1`` THEN
+  X_GEN_TAC (Term`P:real->bool`) THEN
+  POP_ASSUM(MP_TAC o SPEC (Term`\z. P z /\ ~(z = (i:num->real) N)`)) THEN
+  DISCH_THEN(X_CHOOSE_TAC (Term`a:real`)) THEN
+  EXISTS_TAC (Term`abs(a) + abs(i(N:num)) + &1`) THEN
   POP_ASSUM MP_TAC THEN REWRITE_TAC[LT] THEN
-  MP_TAC(REAL_ARITH ``!x v. x < abs(v) + abs(x) + &1``) THEN
-  MP_TAC(REAL_ARITH ``!u v x. x < v ==> x < abs(v) + abs(u) + &1``) THEN
+  MP_TAC(REAL_ARITH (Term`!x v. x < abs(v) + abs(x) + &1`)) THEN
+  MP_TAC(REAL_ARITH (Term`!u v x. x < v ==> x < abs(v) + abs(u) + &1`)) THEN
   MESON_TAC[]);
 
 val POLY_ROOTS_FINITE = store_thm("POLY_ROOTS_FINITE",
- ``!p. ~(poly p = poly []) =
-       ?N i. !x. (poly p(x) = &0) ==> ?n:num. n < N /\ (x = i n)``,
+ (Term`!p. ~(poly p = poly []) =
+       ?N i. !x. (poly p(x) = &0) ==> ?n:num. n < N /\ (x = i n)`),
   GEN_TAC THEN EQ_TAC THEN REWRITE_TAC[POLY_ROOTS_FINITE_LEMMA] THEN
   REWRITE_TAC[FUN_EQ_THM, LEFT_IMP_EXISTS_THM, NOT_FORALL_THM, poly] THEN
-  MP_TAC(GENL [``i:num->real``, ``N:num``]
-   (SPECL [``i:num->real``, ``N:num``, ``\x. poly p x = &0``] FINITE_LEMMA)) THEN
+  MP_TAC(GENL [(Term`i:num->real`), (Term`N:num`)]
+   (SPECL [(Term`i:num->real`), (Term`N:num`), (Term`\x. poly p x = &0`)] FINITE_LEMMA)) THEN
   REWRITE_TAC[] THEN MESON_TAC[REAL_LT_REFL]);
 
 (* ------------------------------------------------------------------------- *)
@@ -603,36 +622,36 @@ val POLY_ROOTS_FINITE = store_thm("POLY_ROOTS_FINITE",
 (* ------------------------------------------------------------------------- *)
 
 val POLY_ENTIRE_LEMMA = store_thm("POLY_ENTIRE_LEMMA",
- ``!p q. ~(poly p = poly []) /\ ~(poly q = poly [])
-         ==> ~(poly (p ** q) = poly [])``,
+ (Term`!p q. ~(poly p = poly []) /\ ~(poly q = poly [])
+         ==> ~(poly (p * q) = poly [])`),
   REPEAT GEN_TAC THEN REWRITE_TAC[POLY_ROOTS_FINITE] THEN
   DISCH_THEN(CONJUNCTS_THEN MP_TAC) THEN
-  DISCH_THEN(X_CHOOSE_THEN ``N2:num`` (X_CHOOSE_TAC ``i2:num->real``)) THEN
-  DISCH_THEN(X_CHOOSE_THEN ``N1:num`` (X_CHOOSE_TAC ``i1:num->real``)) THEN
-  EXISTS_TAC ``N1 + N2:num`` THEN
-  EXISTS_TAC ``\n:num. if n < N1 then i1(n):real else i2(n - N1)`` THEN
-  X_GEN_TAC ``x:real`` THEN REWRITE_TAC[REAL_ENTIRE, POLY_MUL] THEN
-  DISCH_THEN(DISJ_CASES_THEN (ANTE_RES_THEN (X_CHOOSE_TAC ``n:num``))) THENL
-   [EXISTS_TAC ``n:num`` THEN ASM_SIMP_TAC real_ss [],
-    EXISTS_TAC ``N1 + n:num`` THEN ASM_SIMP_TAC real_ss [LT_ADD_LCANCEL]]);
+  DISCH_THEN(X_CHOOSE_THEN (Term`N2:num`) (X_CHOOSE_TAC (Term`i2:num->real`))) THEN
+  DISCH_THEN(X_CHOOSE_THEN (Term`N1:num`) (X_CHOOSE_TAC (Term`i1:num->real`))) THEN
+  EXISTS_TAC (Term`N1 + N2:num`) THEN
+  EXISTS_TAC (Term`\n:num. if n < N1 then i1(n):real else i2(n - N1)`) THEN
+  X_GEN_TAC (Term`x:real`) THEN REWRITE_TAC[REAL_ENTIRE, POLY_MUL] THEN
+  DISCH_THEN(DISJ_CASES_THEN (ANTE_RES_THEN (X_CHOOSE_TAC (Term`n:num`)))) THENL
+   [EXISTS_TAC (Term`n:num`) THEN ASM_SIMP_TAC real_ss [],
+    EXISTS_TAC (Term`N1 + n:num`) THEN ASM_SIMP_TAC real_ss [LT_ADD_LCANCEL]]);
 
 val POLY_ENTIRE = store_thm("POLY_ENTIRE",
- ``!p q. (poly (p ** q) = poly []) = (poly p = poly []) \/ (poly q = poly [])``,
+ (Term`!p q. (poly (p * q) = poly []) = (poly p = poly []) \/ (poly q = poly [])`),
   REPEAT GEN_TAC THEN EQ_TAC THENL
    [MESON_TAC[POLY_ENTIRE_LEMMA],
     REWRITE_TAC[FUN_EQ_THM, POLY_MUL] THEN
     STRIP_TAC THEN ASM_REWRITE_TAC[REAL_MUL_RZERO, REAL_MUL_LZERO, poly]]);
 
 val POLY_MUL_LCANCEL = store_thm("POLY_MUL_LCANCEL",
- ``!p q r. (poly (p ** q) = poly (p ** r)) =
-           (poly p = poly []) \/ (poly q = poly r)``,
+ (Term`!p q r. (poly (p * q) = poly (p * r)) =
+           (poly p = poly []) \/ (poly q = poly r)`),
   let
     val lemma1 = prove
-     (``!p q. (poly (p ++ neg q) = poly []) = (poly p = poly q)``,
+     ((Term`!p q. (poly (p + poly_neg q) = poly []) = (poly p = poly q)`),
       REWRITE_TAC[FUN_EQ_THM, POLY_ADD, POLY_NEG, poly] THEN
-      REWRITE_TAC[REAL_ARITH ``(p + ~q = &0) = (p = q)``])
+      REWRITE_TAC[REAL_ARITH (Term`(p + ~q = &0) = (p = q)`)])
     val lemma2 = prove
-     (``!p q r. poly (p ** q ++ neg(p ** r)) = poly (p ** (q ++ neg(r)))``,
+     ((Term`!p q r. poly (p * q + poly_neg(p * r)) = poly (p * (q + poly_neg(r)))`),
       REWRITE_TAC[FUN_EQ_THM, POLY_ADD, POLY_NEG, POLY_MUL] THEN
       REAL_ARITH_TAC)
   in
@@ -642,23 +661,23 @@ val POLY_MUL_LCANCEL = store_thm("POLY_MUL_LCANCEL",
   end);
 
 val POLY_EXP_EQ_0 = store_thm("POLY_EXP_EQ_0",
- ``!p n. (poly (p pexp n) = poly []) = (poly p = poly []) /\ ~(n = 0)``,
+ (Term`!p n. (poly (p poly_exp n) = poly []) = (poly p = poly []) /\ ~(n = 0)`),
   REPEAT GEN_TAC THEN REWRITE_TAC[FUN_EQ_THM, poly] THEN
   REWRITE_TAC [LEFT_AND_FORALL_THM] THEN AP_TERM_TAC THEN ABS_TAC THEN
-  SPEC_TAC(``n:num``,``n:num``) THEN INDUCT_TAC THEN
-  SIMP_TAC real_ss [poly_pexp, poly, REAL_MUL_RZERO, REAL_ADD_RID,
+  SPEC_TAC((Term`n:num`),(Term`n:num`)) THEN INDUCT_TAC THEN
+  SIMP_TAC real_ss [poly_exp, poly, REAL_MUL_RZERO, REAL_ADD_RID,
     REAL_OF_NUM_EQ, NOT_SUC] THEN
   ASM_REWRITE_TAC[POLY_MUL, poly, REAL_ENTIRE] THEN
   MESON_TAC []);
 
 val POLY_PRIME_EQ_0 = store_thm("POLY_PRIME_EQ_0",
- ``!a. ~(poly [a; &1] = poly [])``,
+ (Term`!a. ~(poly [a; &1] = poly [])`),
   GEN_TAC THEN REWRITE_TAC[FUN_EQ_THM, poly] THEN
-  DISCH_THEN(MP_TAC o SPEC ``&1 - a``) THEN
+  DISCH_THEN(MP_TAC o SPEC (Term`&1 - a`)) THEN
   REAL_ARITH_TAC);
 
 val POLY_EXP_PRIME_EQ_0 = store_thm("POLY_EXP_PRIME_EQ_0",
- ``!a n. ~(poly ([a; &1] pexp n) = poly [])``,
+ (Term`!a n. ~(poly ([a; &1] poly_exp n) = poly [])`),
   MESON_TAC[POLY_EXP_EQ_0, POLY_PRIME_EQ_0]);
 
 (* ------------------------------------------------------------------------- *)
@@ -666,34 +685,34 @@ val POLY_EXP_PRIME_EQ_0 = store_thm("POLY_EXP_PRIME_EQ_0",
 (* ------------------------------------------------------------------------- *)
 
 val POLY_ZERO_LEMMA = store_thm("POLY_ZERO_LEMMA",
- ``!h t. (poly (CONS h t) = poly []) ==> (h = &0) /\ (poly t = poly [])``,
+ (Term`!h t. (poly (CONS h t) = poly []) ==> (h = &0) /\ (poly t = poly [])`),
   let
     val lemma = REWRITE_RULE[FUN_EQ_THM, poly] POLY_ROOTS_FINITE
   in
     REPEAT GEN_TAC
     THEN SIMP_TAC real_ss [FUN_EQ_THM, poly]
-    THEN ASM_CASES_TAC ``h = &0``
+    THEN ASM_CASES_TAC (Term`h = &0`)
     THEN ASM_SIMP_TAC real_ss []
     THENL [
       SIMP_TAC real_ss [REAL_ADD_LID]
       THEN CONV_TAC CONTRAPOS_CONV
       THEN DISCH_THEN(MP_TAC o REWRITE_RULE[lemma])
-      THEN DISCH_THEN(X_CHOOSE_THEN ``N:num`` (X_CHOOSE_TAC ``i:num->real``))
+      THEN DISCH_THEN(X_CHOOSE_THEN (Term`N:num`) (X_CHOOSE_TAC (Term`i:num->real`)))
       THEN MP_TAC
-        (SPECL [``i:num->real``, ``N:num``, ``\x. poly t x = &0``] FINITE_LEMMA)
+        (SPECL [(Term`i:num->real`), (Term`N:num`), (Term`\x. poly t x = &0`)] FINITE_LEMMA)
       THEN ASM_SIMP_TAC real_ss []
-      THEN DISCH_THEN(X_CHOOSE_TAC ``a:real``)
-      THEN EXISTS_TAC ``abs(a) + &1``
-      THEN POP_ASSUM (MP_TAC o SPEC ``abs(a) + &1``)
+      THEN DISCH_THEN(X_CHOOSE_TAC (Term`a:real`))
+      THEN EXISTS_TAC (Term`abs(a) + &1`)
+      THEN POP_ASSUM (MP_TAC o SPEC (Term`abs(a) + &1`))
       THEN REWRITE_TAC [REAL_ENTIRE]
       THEN REAL_ARITH_TAC,
-      EXISTS_TAC ``&0``
+      EXISTS_TAC (Term`&0`)
       THEN ASM_SIMP_TAC real_ss []
     ]
   end);
 
 val POLY_ZERO = store_thm("POLY_ZERO",
- ``!p. (poly p = poly []) = EVERY (\c. c = &0) p``,
+ (Term`!p. (poly p = poly []) = EVERY (\c. c = &0) p`),
   LIST_INDUCT_TAC THEN ASM_REWRITE_TAC[FORALL] THEN EQ_TAC THENL
    [DISCH_THEN(MP_TAC o MATCH_MP POLY_ZERO_LEMMA) THEN ASM_REWRITE_TAC[],
     POP_ASSUM(SUBST1_TAC o SYM) THEN STRIP_TAC THEN
@@ -704,114 +723,117 @@ val POLY_ZERO = store_thm("POLY_ZERO",
 (* ------------------------------------------------------------------------- *)
 
 val POLY_DIFF_AUX_ISZERO = store_thm("POLY_DIFF_AUX_ISZERO",
- ``!p n. EVERY (\c. c = &0) (poly_diff_aux (SUC n) p) =
-         EVERY (\c. c = &0) p``,
+ (Term`!p n. EVERY (\c. c = &0) (poly_diff_aux (SUC n) p) =
+         EVERY (\c. c = &0) p`),
   LIST_INDUCT_TAC THEN ASM_REWRITE_TAC
    [FORALL, poly_diff_aux, REAL_ENTIRE, REAL_OF_NUM_EQ, NOT_SUC]);
 
 
 val POLY_DIFF_ISZERO = store_thm("POLY_DIFF_ISZERO",
- ``!p. (poly (diff p) = poly []) ==> ?h. poly p = poly [h]``,
+ (Term`!p. (poly (diff p) = poly []) ==> ?h. poly p = poly [h]`),
   REWRITE_TAC[POLY_ZERO] THEN
   LIST_INDUCT_TAC THEN ASM_REWRITE_TAC[POLY_DIFF_CLAUSES, FORALL] THENL
-   [EXISTS_TAC ``&0`` THEN REWRITE_TAC[FUN_EQ_THM, poly] THEN REAL_ARITH_TAC,
+   [EXISTS_TAC (Term`&0`) THEN REWRITE_TAC[FUN_EQ_THM, poly] THEN REAL_ARITH_TAC,
     REWRITE_TAC[ONE, POLY_DIFF_AUX_ISZERO] THEN
     REWRITE_TAC[GSYM POLY_ZERO] THEN DISCH_TAC THEN
-    EXISTS_TAC ``h:real`` THEN ASM_REWRITE_TAC[poly, FUN_EQ_THM]]);
+    EXISTS_TAC (Term`h:real`) THEN ASM_REWRITE_TAC[poly, FUN_EQ_THM]]);
 
 val POLY_DIFF_ZERO = store_thm("POLY_DIFF_ZERO",
- ``!p. (poly p = poly []) ==> (poly (diff p) = poly [])``,
+ (Term`!p. (poly p = poly []) ==> (poly (diff p) = poly [])`),
   REWRITE_TAC[POLY_ZERO] THEN
   LIST_INDUCT_TAC THEN REWRITE_TAC[poly_diff, NOT_CONS_NIL] THEN
   REWRITE_TAC[FORALL, TL] THEN
   DISCH_THEN(CONJUNCTS_THEN2 ASSUME_TAC MP_TAC) THEN
-  SPEC_TAC(``1:num``,``n:num``) THEN POP_ASSUM_LIST(K ALL_TAC) THEN
-  SPEC_TAC(``t:real list``,``t:real list``) THEN
+  SPEC_TAC((Term`1:num`),(Term`n:num`)) THEN POP_ASSUM_LIST(K ALL_TAC) THEN
+  SPEC_TAC((Term`t:real list`),(Term`t:real list`)) THEN
   LIST_INDUCT_TAC THEN REWRITE_TAC[FORALL, poly_diff_aux] THEN
   REPEAT STRIP_TAC THEN ASM_REWRITE_TAC[REAL_MUL_RZERO] THEN
   FIRST_ASSUM MATCH_MP_TAC THEN ASM_REWRITE_TAC[]);
 
 val POLY_DIFF_WELLDEF = store_thm("POLY_DIFF_WELLDEF",
- ``!p q. (poly p = poly q) ==> (poly (diff p) = poly (diff q))``,
-  REPEAT STRIP_TAC THEN MP_TAC(SPEC ``p ++ neg(q)`` POLY_DIFF_ZERO) THEN
+ (Term`!p q. (poly p = poly q) ==> (poly (diff p) = poly (diff q))`),
+  REPEAT STRIP_TAC THEN MP_TAC(SPEC (Term`p + poly_neg(q)`) POLY_DIFF_ZERO) THEN
   REWRITE_TAC[FUN_EQ_THM, POLY_DIFF_ADD, POLY_DIFF_NEG, POLY_ADD] THEN
-  ASM_REWRITE_TAC[POLY_NEG, poly, REAL_ARITH ``a + ~a = &0``] THEN
-  REWRITE_TAC[REAL_ARITH ``(a + ~b = &0) = (a = b)``]);
+  ASM_REWRITE_TAC[POLY_NEG, poly, REAL_ARITH (Term`a + ~a = &0`)] THEN
+  REWRITE_TAC[REAL_ARITH (Term`(a + ~b = &0) = (a = b)`)]);
 
 (* ------------------------------------------------------------------------- *)
 (* Basics of divisibility.                                                   *)
 (* ------------------------------------------------------------------------- *)
 
 val poly_divides = new_infixl_definition ("poly_divides",
-  ``$poly_divides p1 p2 = ?q. poly p2 = poly (p1 ** q)``, 475);
+  (Term`$poly_divides p1 p2 = ?q. poly p2 = poly (p1 * q)`), 475);
 
 val POLY_PRIMES = store_thm("POLY_PRIMES",
- ``!a p q. [a; &1] poly_divides (p ** q) = [a; &1] poly_divides p \/ [a; &1] poly_divides q``,
-  REPEAT GEN_TAC THEN REWRITE_TAC[poly_divides, POLY_MUL, FUN_EQ_THM, poly] THEN
-  REWRITE_TAC[REAL_MUL_RZERO, REAL_ADD_RID, REAL_MUL_RID] THEN EQ_TAC THENL
-   [DISCH_THEN(X_CHOOSE_THEN ``r:real list`` (MP_TAC o SPEC ``~a``)) THEN
-    REWRITE_TAC[REAL_ENTIRE, GSYM real_sub, REAL_SUB_REFL, REAL_MUL_LZERO] THEN
+ (Term`!a p q. [a; &1] poly_divides (p * q) 
+                           = 
+               [a; &1] poly_divides p \/ [a; &1] poly_divides q`),
+ REPEAT GEN_TAC THEN REWRITE_TAC[poly_divides, POLY_MUL, FUN_EQ_THM, poly] THEN
+ REWRITE_TAC[REAL_MUL_RZERO, REAL_ADD_RID, REAL_MUL_RID] THEN EQ_TAC THENL
+ [DISCH_THEN(X_CHOOSE_THEN (Term`r:real list`) 
+  (MP_TAC o SPEC (Term`~a:real`))) THEN
+   REWRITE_TAC[REAL_ENTIRE, GSYM real_sub, REAL_SUB_REFL, REAL_MUL_LZERO] THEN
     DISCH_THEN DISJ_CASES_TAC THENL [DISJ1_TAC, DISJ2_TAC] THEN
     (POP_ASSUM(MP_TAC o REWRITE_RULE[POLY_LINEAR_DIVIDES]) THEN
      REWRITE_TAC[REAL_NEG_NEG] THEN
      DISCH_THEN(DISJ_CASES_THEN2 SUBST_ALL_TAC
-        (X_CHOOSE_THEN ``s:real list`` SUBST_ALL_TAC)) THENL
-      [EXISTS_TAC ``[]:real list`` THEN REWRITE_TAC[poly, REAL_MUL_RZERO],
-       EXISTS_TAC ``s:real list`` THEN GEN_TAC THEN
+        (X_CHOOSE_THEN (Term`s:real list`) SUBST_ALL_TAC)) THENL
+      [EXISTS_TAC (Term`[]:real list`) THEN REWRITE_TAC[poly, REAL_MUL_RZERO],
+       EXISTS_TAC (Term`s:real list`) THEN GEN_TAC THEN
        REWRITE_TAC[POLY_MUL, poly] THEN REAL_ARITH_TAC]),
-    DISCH_THEN(DISJ_CASES_THEN(X_CHOOSE_TAC ``s:real list``)) THEN
+    DISCH_THEN(DISJ_CASES_THEN(X_CHOOSE_TAC (Term`s:real list`))) THEN
     ASM_REWRITE_TAC[] THENL
-     [EXISTS_TAC ``s ** q``, EXISTS_TAC ``p ** s``] THEN
+     [EXISTS_TAC (Term`s * q`), EXISTS_TAC (Term`p * s`)] THEN
     GEN_TAC THEN REWRITE_TAC[POLY_MUL] THEN REAL_ARITH_TAC]);
 
 val POLY_DIVIDES_REFL = store_thm("POLY_DIVIDES_REFL",
- ``!p. p poly_divides p``,
-  GEN_TAC THEN REWRITE_TAC[poly_divides] THEN EXISTS_TAC ``[&1]`` THEN
+ (Term`!p. p poly_divides p`),
+  GEN_TAC THEN REWRITE_TAC[poly_divides] THEN EXISTS_TAC (Term`[&1]`) THEN
   REWRITE_TAC[FUN_EQ_THM, POLY_MUL, poly] THEN REAL_ARITH_TAC);
 
 val POLY_DIVIDES_TRANS = store_thm("POLY_DIVIDES_TRANS",
- ``!p q r. p poly_divides q /\ q poly_divides r ==> p poly_divides r``,
+ (Term`!p q r. p poly_divides q /\ q poly_divides r ==> p poly_divides r`),
   REPEAT GEN_TAC THEN REWRITE_TAC[poly_divides] THEN
   DISCH_THEN(CONJUNCTS_THEN MP_TAC) THEN
-  DISCH_THEN(X_CHOOSE_THEN ``s:real list`` ASSUME_TAC) THEN
-  DISCH_THEN(X_CHOOSE_THEN ``t:real list`` ASSUME_TAC) THEN
-  EXISTS_TAC ``t ** s`` THEN
+  DISCH_THEN(X_CHOOSE_THEN (Term`s:real list`) ASSUME_TAC) THEN
+  DISCH_THEN(X_CHOOSE_THEN (Term`t:real list`) ASSUME_TAC) THEN
+  EXISTS_TAC (Term`t * s`) THEN
   ASM_REWRITE_TAC[FUN_EQ_THM, POLY_MUL, REAL_MUL_ASSOC]);
 
 val POLY_DIVIDES_EXP = store_thm("POLY_DIVIDES_EXP",
- ``!p m n. m <= n ==> (p pexp m) poly_divides (p pexp n)``,
+ (Term`!p m n. m <= n ==> (p poly_exp m) poly_divides (p poly_exp n)`),
   REPEAT GEN_TAC THEN REWRITE_TAC[LE_EXISTS] THEN
-  DISCH_THEN(X_CHOOSE_THEN ``d:num`` SUBST1_TAC) THEN
-  SPEC_TAC(``d:num``,``d:num``) THEN INDUCT_TAC THEN
+  DISCH_THEN(X_CHOOSE_THEN (Term`d:num`) SUBST1_TAC) THEN
+  SPEC_TAC((Term`d:num`),(Term`d:num`)) THEN INDUCT_TAC THEN
   REWRITE_TAC[ADD_CLAUSES, POLY_DIVIDES_REFL] THEN
   MATCH_MP_TAC POLY_DIVIDES_TRANS THEN
-  EXISTS_TAC ``p pexp (m + d)`` THEN ASM_REWRITE_TAC[] THEN
-  REWRITE_TAC[poly_divides] THEN EXISTS_TAC ``p:real list`` THEN
-  REWRITE_TAC[poly_pexp, FUN_EQ_THM, POLY_MUL] THEN
+  EXISTS_TAC (Term`p poly_exp (m + d)`) THEN ASM_REWRITE_TAC[] THEN
+  REWRITE_TAC[poly_divides] THEN EXISTS_TAC (Term`p:real list`) THEN
+  REWRITE_TAC[poly_exp, FUN_EQ_THM, POLY_MUL] THEN
   REAL_ARITH_TAC);
 
 val POLY_EXP_DIVIDES = store_thm("POLY_EXP_DIVIDES",
- ``!p q m n.
-      (p pexp n) poly_divides q /\ m <= n ==> (p pexp m) poly_divides q``,
+ (Term`!p q m n.
+      (p poly_exp n) poly_divides q /\ m <= n ==> (p poly_exp m) poly_divides q`),
   MESON_TAC[POLY_DIVIDES_TRANS, POLY_DIVIDES_EXP]);
 
 val POLY_DIVIDES_ADD = store_thm("POLY_DIVIDES_ADD",
- ``!p q r. p poly_divides q /\ p poly_divides r ==> p poly_divides (q ++ r)``,
+ (Term`!p q r. p poly_divides q /\ p poly_divides r ==> p poly_divides (q + r)`),
   REPEAT GEN_TAC THEN REWRITE_TAC[poly_divides] THEN
   DISCH_THEN(CONJUNCTS_THEN MP_TAC) THEN
-  DISCH_THEN(X_CHOOSE_THEN ``s:real list`` ASSUME_TAC) THEN
-  DISCH_THEN(X_CHOOSE_THEN ``t:real list`` ASSUME_TAC) THEN
-  EXISTS_TAC ``t ++ s`` THEN
+  DISCH_THEN(X_CHOOSE_THEN (Term`s:real list`) ASSUME_TAC) THEN
+  DISCH_THEN(X_CHOOSE_THEN (Term`t:real list`) ASSUME_TAC) THEN
+  EXISTS_TAC (Term`t + s`) THEN
   ASM_REWRITE_TAC[FUN_EQ_THM, POLY_ADD, POLY_MUL] THEN
   REAL_ARITH_TAC);
 
 val POLY_DIVIDES_SUB = store_thm("POLY_DIVIDES_SUB",
- ``!p q r. p poly_divides q /\ p poly_divides (q ++ r) ==> p poly_divides r``,
+ (Term`!p q r. p poly_divides q /\ p poly_divides (q + r) ==> p poly_divides r`),
   REPEAT GEN_TAC THEN REWRITE_TAC[poly_divides] THEN
   DISCH_THEN(CONJUNCTS_THEN MP_TAC) THEN
-  DISCH_THEN(X_CHOOSE_THEN ``s:real list`` ASSUME_TAC) THEN
-  DISCH_THEN(X_CHOOSE_THEN ``t:real list`` ASSUME_TAC) THEN
-  EXISTS_TAC ``s ++ neg(t)`` THEN
+  DISCH_THEN(X_CHOOSE_THEN (Term`s:real list`) ASSUME_TAC) THEN
+  DISCH_THEN(X_CHOOSE_THEN (Term`t:real list`) ASSUME_TAC) THEN
+  EXISTS_TAC (Term`s + poly_neg(t)`) THEN
   POP_ASSUM_LIST(MP_TAC o end_itlist CONJ) THEN
   REWRITE_TAC[FUN_EQ_THM, POLY_ADD, POLY_MUL, POLY_NEG] THEN
   DISCH_THEN(STRIP_ASSUME_TAC o GSYM) THEN
@@ -819,20 +841,20 @@ val POLY_DIVIDES_SUB = store_thm("POLY_DIVIDES_SUB",
   ASM_REWRITE_TAC[] THEN REAL_ARITH_TAC);
 
 val POLY_DIVIDES_SUB2 = store_thm("POLY_DIVIDES_SUB2",
- ``!p q r. p poly_divides r /\ p poly_divides (q ++ r) ==> p poly_divides q``,
+ (Term`!p q r. p poly_divides r /\ p poly_divides (q + r) ==> p poly_divides q`),
   REPEAT STRIP_TAC THEN MATCH_MP_TAC POLY_DIVIDES_SUB THEN
-  EXISTS_TAC ``r:real list`` THEN ASM_REWRITE_TAC[] THEN
-  UNDISCH_TAC ``p poly_divides (q ++ r)`` THEN
+  EXISTS_TAC (Term`r:real list`) THEN ASM_REWRITE_TAC[] THEN
+  UNDISCH_TAC (Term`p poly_divides (q + r)`) THEN
   REWRITE_TAC[poly_divides, POLY_ADD, FUN_EQ_THM, POLY_MUL] THEN
-  DISCH_THEN(X_CHOOSE_TAC ``s:real list``) THEN
-  EXISTS_TAC ``s:real list`` THEN
-  X_GEN_TAC ``x:real`` THEN POP_ASSUM(MP_TAC o SPEC ``x:real``) THEN
+  DISCH_THEN(X_CHOOSE_TAC (Term`s:real list`)) THEN
+  EXISTS_TAC (Term`s:real list`) THEN
+  X_GEN_TAC (Term`x:real`) THEN POP_ASSUM(MP_TAC o SPEC (Term`x:real`)) THEN
   REAL_ARITH_TAC);
 
 val POLY_DIVIDES_ZERO = store_thm("POLY_DIVIDES_ZERO",
- ``!p q. (poly p = poly []) ==> q poly_divides p``,
+ (Term`!p q. (poly p = poly []) ==> q poly_divides p`),
   REPEAT GEN_TAC THEN DISCH_TAC THEN REWRITE_TAC[poly_divides] THEN
-  EXISTS_TAC ``[]:real list`` THEN
+  EXISTS_TAC (Term`[]:real list`) THEN
   ASM_REWRITE_TAC[FUN_EQ_THM, POLY_MUL, poly, REAL_MUL_RZERO]);
 
 (* ------------------------------------------------------------------------- *)
@@ -840,83 +862,83 @@ val POLY_DIVIDES_ZERO = store_thm("POLY_DIVIDES_ZERO",
 (* ------------------------------------------------------------------------- *)
 
 val POLY_ORDER_EXISTS = store_thm("POLY_ORDER_EXISTS",
- ``!a d. !p. (LENGTH p = d) /\ ~(poly p = poly [])
-             ==> ?n. ([~a; &1] pexp n) poly_divides p /\
-                     ~(([~a; &1] pexp (SUC n)) poly_divides p)``,
+ (Term`!a d. !p. (LENGTH p = d) /\ ~(poly p = poly [])
+             ==> ?n. ([~a; &1] poly_exp n) poly_divides p /\
+                     ~(([~a; &1] poly_exp (SUC n)) poly_divides p)`),
   GEN_TAC
   THEN (STRIP_ASSUME_TAC o prove_rec_fn_exists num_Axiom)
-    ``(!p q. mulexp 0 p q = q) /\
-     (!p q n. mulexp (SUC n) p q = p ** (mulexp n p q))``
+    (Term`(!p q. mulexp 0 p q = q) /\
+     (!p q n. mulexp (SUC n) p q = p * (mulexp n p q))`)
   THEN SUBGOAL_THEN
-    ``!d. !p. (LENGTH p = d) /\ ~(poly p = poly [])
+    (Term`!d. !p. (LENGTH p = d) /\ ~(poly p = poly [])
            ==> ?n q. (p = mulexp (n:num) [~a; &1] q) /\
-                     ~(poly q a = &0)`` MP_TAC
+                     ~(poly q a = &0)`) MP_TAC
   THENL [ INDUCT_TAC THENL [SIMP_TAC real_ss [LENGTH_NIL], ALL_TAC]
-    THEN X_GEN_TAC ``p:real list``
-    THEN ASM_CASES_TAC ``poly p a = &0``
+    THEN X_GEN_TAC (Term`p:real list`)
+    THEN ASM_CASES_TAC (Term`poly p a = &0`)
     THENL [
       STRIP_TAC
-      THEN UNDISCH_TAC ``poly p a = &0``
+      THEN UNDISCH_TAC (Term`poly p a = &0`)
       THEN DISCH_THEN(MP_TAC o REWRITE_RULE[POLY_LINEAR_DIVIDES])
       THEN DISCH_THEN(DISJ_CASES_THEN MP_TAC)
       THENL [
         ASM_MESON_TAC[],
         ALL_TAC
       ]
-      THEN DISCH_THEN(X_CHOOSE_THEN ``q:real list`` SUBST_ALL_TAC)
+      THEN DISCH_THEN(X_CHOOSE_THEN (Term`q:real list`) SUBST_ALL_TAC)
       THEN UNDISCH_TAC
-        ``!p. (LENGTH p = d) /\ ~(poly p = poly [])
+        (Term`!p. (LENGTH p = d) /\ ~(poly p = poly [])
          ==> ?n q. (p = mulexp (n:num) [~a; &1] q) /\
-                   ~(poly q a = &0)``
-      THEN DISCH_THEN(MP_TAC o SPEC ``q:real list``)
+                   ~(poly q a = &0)`)
+      THEN DISCH_THEN(MP_TAC o SPEC (Term`q:real list`))
       THEN RULE_ASSUM_TAC(REWRITE_RULE[POLY_LENGTH_MUL, POLY_ENTIRE,
         DE_MORGAN_THM, SUC_INJ])
       THEN ASM_REWRITE_TAC[]
-      THEN DISCH_THEN(X_CHOOSE_THEN ``n:num``
-        (X_CHOOSE_THEN ``s:real list`` STRIP_ASSUME_TAC))
-      THEN EXISTS_TAC ``SUC n``
-      THEN EXISTS_TAC ``s:real list``
+      THEN DISCH_THEN(X_CHOOSE_THEN (Term`n:num`)
+        (X_CHOOSE_THEN (Term`s:real list`) STRIP_ASSUME_TAC))
+      THEN EXISTS_TAC (Term`SUC n`)
+      THEN EXISTS_TAC (Term`s:real list`)
       THEN ASM_REWRITE_TAC[],
       STRIP_TAC
-      THEN EXISTS_TAC ``0:num``
-      THEN EXISTS_TAC ``p:real list``
+      THEN EXISTS_TAC (Term`0:num`)
+      THEN EXISTS_TAC (Term`p:real list`)
       THEN ASM_REWRITE_TAC[]
     ],
     DISCH_TAC
     THEN REPEAT GEN_TAC
     THEN DISCH_THEN(ANTE_RES_THEN MP_TAC)
-    THEN DISCH_THEN(X_CHOOSE_THEN ``n:num``
-      (X_CHOOSE_THEN ``s:real list`` STRIP_ASSUME_TAC))
-    THEN EXISTS_TAC ``n:num``
+    THEN DISCH_THEN(X_CHOOSE_THEN (Term`n:num`)
+      (X_CHOOSE_THEN (Term`s:real list`) STRIP_ASSUME_TAC))
+    THEN EXISTS_TAC (Term`n:num`)
     THEN ASM_REWRITE_TAC[]
     THEN REWRITE_TAC[poly_divides]
     THEN CONJ_TAC
     THENL [
-      EXISTS_TAC ``s:real list``
-      THEN SPEC_TAC(``n:num``,``n:num``)
+      EXISTS_TAC (Term`s:real list`)
+      THEN SPEC_TAC((Term`n:num`),(Term`n:num`))
       THEN INDUCT_TAC
-      THEN ASM_REWRITE_TAC[poly_pexp, FUN_EQ_THM, POLY_MUL, poly]
+      THEN ASM_REWRITE_TAC[poly_exp, FUN_EQ_THM, POLY_MUL, poly]
       THEN REAL_ARITH_TAC,
-      DISCH_THEN(X_CHOOSE_THEN ``r:real list`` MP_TAC)
-      THEN SPEC_TAC(``n:num``,``n:num``)
+      DISCH_THEN(X_CHOOSE_THEN (Term`r:real list`) MP_TAC)
+      THEN SPEC_TAC((Term`n:num`),(Term`n:num`))
       THEN INDUCT_TAC
       THEN ASM_SIMP_TAC bool_ss []
       THENL [
-        UNDISCH_TAC ``~(poly s a = &0)``
+        UNDISCH_TAC (Term`~(poly s a = &0)`)
         THEN CONV_TAC CONTRAPOS_CONV
         THEN REWRITE_TAC[]
         THEN DISCH_THEN SUBST1_TAC
-        THEN REWRITE_TAC[poly, poly_pexp, POLY_MUL]
+        THEN REWRITE_TAC[poly, poly_exp, POLY_MUL]
         THEN REAL_ARITH_TAC,
         REWRITE_TAC[]
         THEN ONCE_ASM_REWRITE_TAC[]
-        THEN ONCE_REWRITE_TAC[poly_pexp]
+        THEN ONCE_REWRITE_TAC[poly_exp]
         THEN REWRITE_TAC[GSYM POLY_MUL_ASSOC, POLY_MUL_LCANCEL]
         THEN REWRITE_TAC[DE_MORGAN_THM]
         THEN CONJ_TAC
         THENL [
           REWRITE_TAC[FUN_EQ_THM]
-          THEN DISCH_THEN(MP_TAC o SPEC ``a + &1``)
+          THEN DISCH_THEN(MP_TAC o SPEC (Term`a + &1`))
           THEN REWRITE_TAC[poly]
           THEN REAL_ARITH_TAC,
           DISCH_THEN(ANTE_RES_THEN MP_TAC)
@@ -927,9 +949,9 @@ val POLY_ORDER_EXISTS = store_thm("POLY_ORDER_EXISTS",
   ]);
 
 val POLY_ORDER = store_thm("POLY_ORDER",
- ``!p a. ~(poly p = poly [])
-         ==> ?!n. ([~a; &1] pexp n) poly_divides p /\
-                      ~(([~a; &1] pexp (SUC n)) poly_divides p)``,
+ (Term`!p a. ~(poly p = poly [])
+         ==> ?!n. ([~a; &1] poly_exp n) poly_divides p /\
+                      ~(([~a; &1] poly_exp (SUC n)) poly_divides p)`),
   MESON_TAC[POLY_ORDER_EXISTS, POLY_EXP_DIVIDES, LE_SUC_LT, LT_CASES]);
 
 (* ------------------------------------------------------------------------- *)
@@ -937,20 +959,20 @@ val POLY_ORDER = store_thm("POLY_ORDER",
 (* ------------------------------------------------------------------------- *)
 
 val poly_order = new_definition ("poly_order",
-  ``poly_order a p = @n. ([~a; &1] pexp n) poly_divides p /\
-                   ~(([~a; &1] pexp (SUC n)) poly_divides p)``);
+  (Term`poly_order a p = @n. ([~a; &1] poly_exp n) poly_divides p /\
+                   ~(([~a; &1] poly_exp (SUC n)) poly_divides p)`));
 
 val ORDER = store_thm("ORDER",
- ``!p a n. ([~a; &1] pexp n) poly_divides p /\
-           ~(([~a; &1] pexp (SUC n)) poly_divides p) =
+ (Term`!p a n. ([~a; &1] poly_exp n) poly_divides p /\
+           ~(([~a; &1] poly_exp (SUC n)) poly_divides p) =
            (n = poly_order a p) /\
-           ~(poly p = poly [])``,
+           ~(poly p = poly [])`),
   REPEAT GEN_TAC THEN REWRITE_TAC[poly_order] THEN
   EQ_TAC THEN STRIP_TAC THENL
-   [SUBGOAL_THEN ``~(poly p = poly [])`` ASSUME_TAC THENL
+   [SUBGOAL_THEN (Term`~(poly p = poly [])`) ASSUME_TAC THENL
      [FIRST_ASSUM(UNDISCH_TAC o assert is_neg o concl) THEN
       CONV_TAC CONTRAPOS_CONV THEN REWRITE_TAC[poly_divides] THEN
-      DISCH_THEN SUBST1_TAC THEN EXISTS_TAC ``[]:real list`` THEN
+      DISCH_THEN SUBST1_TAC THEN EXISTS_TAC (Term`[]:real list`) THEN
       REWRITE_TAC[FUN_EQ_THM, POLY_MUL, poly, REAL_MUL_RZERO],
       ASM_REWRITE_TAC[] THEN CONV_TAC SYM_CONV THEN
       MATCH_MP_TAC SELECT_UNIQUE THEN REWRITE_TAC[]],
@@ -958,66 +980,66 @@ val ORDER = store_thm("ORDER",
   ASM_MESON_TAC[POLY_ORDER]);
 
 val ORDER_THM = store_thm("ORDER_THM",
- ``!p a. ~(poly p = poly [])
-         ==> ([~a; &1] pexp (poly_order a p)) poly_divides p /\
-             ~(([~a; &1] pexp (SUC(poly_order a p))) poly_divides p)``,
+ (Term`!p a. ~(poly p = poly [])
+         ==> ([~a; &1] poly_exp (poly_order a p)) poly_divides p /\
+             ~(([~a; &1] poly_exp (SUC(poly_order a p))) poly_divides p)`),
   MESON_TAC[ORDER]);
 
 val ORDER_UNIQUE = store_thm("ORDER_UNIQUE",
- ``!p a n. ~(poly p = poly []) /\
-           ([~a; &1] pexp n) poly_divides p /\
-           ~(([~a; &1] pexp (SUC n)) poly_divides p)
-           ==> (n = poly_order a p)``,
+ (Term`!p a n. ~(poly p = poly []) /\
+           ([~a; &1] poly_exp n) poly_divides p /\
+           ~(([~a; &1] poly_exp (SUC n)) poly_divides p)
+           ==> (n = poly_order a p)`),
   MESON_TAC[ORDER]);
 
 val ORDER_POLY = store_thm("ORDER_POLY",
- ``!p q a. (poly p = poly q) ==> (poly_order a p = poly_order a q)``,
+ (Term`!p q a. (poly p = poly q) ==> (poly_order a p = poly_order a q)`),
   REPEAT STRIP_TAC THEN
   ASM_REWRITE_TAC[poly_order, poly_divides, FUN_EQ_THM, POLY_MUL]);
 
 val ORDER_ROOT = store_thm("ORDER_ROOT",
- ``!p a. (poly p a = &0) = (poly p = poly []) \/ ~(poly_order a p = 0)``,
-  REPEAT GEN_TAC THEN ASM_CASES_TAC ``poly p = poly []`` THEN
+ (Term`!p a. (poly p a = &0) = (poly p = poly []) \/ ~(poly_order a p = 0)`),
+  REPEAT GEN_TAC THEN ASM_CASES_TAC (Term`poly p = poly []`) THEN
   ASM_REWRITE_TAC[poly] THEN EQ_TAC THENL
    [DISCH_THEN(MP_TAC o REWRITE_RULE[POLY_LINEAR_DIVIDES]) THEN
-    ASM_CASES_TAC ``p:real list = []`` THENL [ASM_MESON_TAC[], ALL_TAC] THEN
+    ASM_CASES_TAC (Term`p:real list = []`) THENL [ASM_MESON_TAC[], ALL_TAC] THEN
     ASM_REWRITE_TAC[] THEN
-    DISCH_THEN(X_CHOOSE_THEN ``q:real list`` SUBST_ALL_TAC) THEN DISCH_TAC THEN
-    FIRST_ASSUM(MP_TAC o SPEC ``a:real`` o MATCH_MP ORDER_THM) THEN
-    ASM_REWRITE_TAC[poly_pexp, DE_MORGAN_THM] THEN DISJ2_TAC THEN
-    REWRITE_TAC[poly_divides] THEN EXISTS_TAC ``q:real list`` THEN
+    DISCH_THEN(X_CHOOSE_THEN (Term`q:real list`) SUBST_ALL_TAC) THEN DISCH_TAC THEN
+    FIRST_ASSUM(MP_TAC o SPEC (Term`a:real`) o MATCH_MP ORDER_THM) THEN
+    ASM_REWRITE_TAC[poly_exp, DE_MORGAN_THM] THEN DISJ2_TAC THEN
+    REWRITE_TAC[poly_divides] THEN EXISTS_TAC (Term`q:real list`) THEN
     REWRITE_TAC[FUN_EQ_THM, POLY_MUL, poly] THEN REAL_ARITH_TAC,
     DISCH_TAC THEN
-    FIRST_ASSUM(MP_TAC o SPEC ``a:real`` o MATCH_MP ORDER_THM) THEN
-    UNDISCH_TAC ``~(poly_order a p = 0)`` THEN
-    SPEC_TAC(``poly_order a p``,``n:num``) THEN
-    INDUCT_TAC THEN ASM_REWRITE_TAC[poly_pexp, NOT_SUC] THEN
+    FIRST_ASSUM(MP_TAC o SPEC (Term`a:real`) o MATCH_MP ORDER_THM) THEN
+    UNDISCH_TAC (Term`~(poly_order a p = 0)`) THEN
+    SPEC_TAC((Term`poly_order a p`),(Term`n:num`)) THEN
+    INDUCT_TAC THEN ASM_REWRITE_TAC[poly_exp, NOT_SUC] THEN
     DISCH_THEN(MP_TAC o CONJUNCT1) THEN REWRITE_TAC[poly_divides] THEN
-    DISCH_THEN(X_CHOOSE_THEN ``s:real list`` SUBST1_TAC) THEN
+    DISCH_THEN(X_CHOOSE_THEN (Term`s:real list`) SUBST1_TAC) THEN
     REWRITE_TAC[POLY_MUL, poly] THEN REAL_ARITH_TAC]);
 
 val ORDER_DIVIDES = store_thm("ORDER_DIVIDES",
- ``!p a n. ([~a; &1] pexp n) poly_divides p =
-           (poly p = poly []) \/ n <= poly_order a p``,
-  REPEAT GEN_TAC THEN ASM_CASES_TAC ``poly p = poly []`` THEN
+ (Term`!p a n. ([~a; &1] poly_exp n) poly_divides p =
+           (poly p = poly []) \/ n <= poly_order a p`),
+  REPEAT GEN_TAC THEN ASM_CASES_TAC (Term`poly p = poly []`) THEN
   ASM_REWRITE_TAC[] THENL
-   [ASM_REWRITE_TAC[poly_divides] THEN EXISTS_TAC ``[]:real list`` THEN
+   [ASM_REWRITE_TAC[poly_divides] THEN EXISTS_TAC (Term`[]:real list`) THEN
     REWRITE_TAC[FUN_EQ_THM, POLY_MUL, poly, REAL_MUL_RZERO],
     ASM_MESON_TAC[ORDER_THM, POLY_EXP_DIVIDES, NOT_LE, LE_SUC_LT]]);
 
 val ORDER_DECOMP = store_thm("ORDER_DECOMP",
- ``!p a. ~(poly p = poly [])
-         ==> ?q. (poly p = poly (([~a; &1] pexp (poly_order a p)) ** q)) /\
-                 ~([~a; &1] poly_divides q)``,
+ (Term`!p a. ~(poly p = poly [])
+         ==> ?q. (poly p = poly (([~a; &1] poly_exp (poly_order a p)) * q)) /\
+                 ~([~a; &1] poly_divides q)`),
   REPEAT STRIP_TAC THEN FIRST_ASSUM(MP_TAC o MATCH_MP ORDER_THM) THEN
-  DISCH_THEN(CONJUNCTS_THEN2 MP_TAC ASSUME_TAC o SPEC ``a:real``) THEN
-  DISCH_THEN(X_CHOOSE_TAC ``q:real list`` o REWRITE_RULE[poly_divides]) THEN
-  EXISTS_TAC ``q:real list`` THEN ASM_REWRITE_TAC[] THEN
-  DISCH_THEN(X_CHOOSE_TAC ``r: real list`` o REWRITE_RULE[poly_divides]) THEN
-  UNDISCH_TAC ``~([~ a; &1] pexp SUC (poly_order a p) poly_divides p)`` THEN
+  DISCH_THEN(CONJUNCTS_THEN2 MP_TAC ASSUME_TAC o SPEC (Term`a:real`)) THEN
+  DISCH_THEN(X_CHOOSE_TAC (Term`q:real list`) o REWRITE_RULE[poly_divides]) THEN
+  EXISTS_TAC (Term`q:real list`) THEN ASM_REWRITE_TAC[] THEN
+  DISCH_THEN(X_CHOOSE_TAC (Term`r: real list`) o REWRITE_RULE[poly_divides]) THEN
+  UNDISCH_TAC (Term`~([~ a; &1] poly_exp SUC (poly_order a p) poly_divides p)`) THEN
   ASM_REWRITE_TAC[] THEN REWRITE_TAC[poly_divides] THEN
-  EXISTS_TAC ``r:real list`` THEN
-  ASM_REWRITE_TAC[POLY_MUL, FUN_EQ_THM, poly_pexp] THEN
+  EXISTS_TAC (Term`r:real list`) THEN
+  ASM_REWRITE_TAC[POLY_MUL, FUN_EQ_THM, poly_exp] THEN
   REAL_ARITH_TAC);
 
 (* ------------------------------------------------------------------------- *)
@@ -1025,14 +1047,14 @@ val ORDER_DECOMP = store_thm("ORDER_DECOMP",
 (* ------------------------------------------------------------------------- *)
 
 val ORDER_MUL = store_thm("ORDER_MUL",
- ``!a p q. ~(poly (p ** q) = poly []) ==>
-           (poly_order a (p ** q) = poly_order a p + poly_order a q)``,
+ (Term`!a p q. ~(poly (p * q) = poly []) ==>
+           (poly_order a (p * q) = poly_order a p + poly_order a q)`),
   REPEAT GEN_TAC
   THEN DISCH_THEN(fn th => ASSUME_TAC th THEN MP_TAC th)
   THEN REWRITE_TAC[POLY_ENTIRE, DE_MORGAN_THM]
   THEN STRIP_TAC
-  THEN SUBGOAL_THEN ``(poly_order a p + poly_order a q
-    = poly_order a (p ** q)) /\ ~(poly (p ** q) = poly [])`` MP_TAC
+  THEN SUBGOAL_THEN (Term`(poly_order a p + poly_order a q
+    = poly_order a (p * q)) /\ ~(poly (p * q) = poly [])`) MP_TAC
   THENL [
     ALL_TAC,
     MESON_TAC[]
@@ -1040,40 +1062,40 @@ val ORDER_MUL = store_thm("ORDER_MUL",
   THEN REWRITE_TAC[GSYM ORDER]
   THEN CONJ_TAC
   THENL [
-    MP_TAC(CONJUNCT1 (SPEC ``a:real``
-      (MATCH_MP ORDER_THM (ASSUME ``~(poly p = poly [])``))))
-    THEN DISCH_THEN(X_CHOOSE_TAC ``r: real list`` o REWRITE_RULE[poly_divides])
-    THEN MP_TAC(CONJUNCT1 (SPEC ``a:real``
-      (MATCH_MP ORDER_THM (ASSUME ``~(poly q = poly [])``))))
-    THEN DISCH_THEN(X_CHOOSE_TAC ``s: real list`` o REWRITE_RULE[poly_divides])
+    MP_TAC(CONJUNCT1 (SPEC (Term`a:real`)
+      (MATCH_MP ORDER_THM (ASSUME (Term`~(poly p = poly [])`)))))
+    THEN DISCH_THEN(X_CHOOSE_TAC (Term`r: real list`) o REWRITE_RULE[poly_divides])
+    THEN MP_TAC(CONJUNCT1 (SPEC (Term`a:real`)
+      (MATCH_MP ORDER_THM (ASSUME (Term`~(poly q = poly [])`)))))
+    THEN DISCH_THEN(X_CHOOSE_TAC (Term`s: real list`) o REWRITE_RULE[poly_divides])
     THEN REWRITE_TAC[poly_divides, FUN_EQ_THM]
-    THEN EXISTS_TAC ``s ** r``
+    THEN EXISTS_TAC (Term`s * r`)
     THEN ASM_REWRITE_TAC[POLY_MUL, POLY_EXP_ADD]
     THEN REAL_ARITH_TAC,
-    X_CHOOSE_THEN ``r: real list`` STRIP_ASSUME_TAC
-    (SPEC ``a:real`` (MATCH_MP ORDER_DECOMP (ASSUME ``~(poly p = poly [])``)))
-    THEN X_CHOOSE_THEN ``s: real list`` STRIP_ASSUME_TAC
-    (SPEC ``a:real`` (MATCH_MP ORDER_DECOMP (ASSUME ``~(poly q = poly [])``)))
-    THEN ASM_REWRITE_TAC[poly_divides, FUN_EQ_THM, POLY_EXP_ADD, POLY_MUL, poly_pexp]
-    THEN DISCH_THEN(X_CHOOSE_THEN ``t:real list`` STRIP_ASSUME_TAC)
-    THEN SUBGOAL_THEN ``[~a; &1] poly_divides (r ** s)`` MP_TAC
+    X_CHOOSE_THEN (Term`r: real list`) STRIP_ASSUME_TAC
+    (SPEC (Term`a:real`) (MATCH_MP ORDER_DECOMP (ASSUME (Term`~(poly p = poly [])`))))
+    THEN X_CHOOSE_THEN (Term`s: real list`) STRIP_ASSUME_TAC
+    (SPEC (Term`a:real`) (MATCH_MP ORDER_DECOMP (ASSUME (Term`~(poly q = poly [])`))))
+    THEN ASM_REWRITE_TAC[poly_divides, FUN_EQ_THM, POLY_EXP_ADD, POLY_MUL, poly_exp]
+    THEN DISCH_THEN(X_CHOOSE_THEN (Term`t:real list`) STRIP_ASSUME_TAC)
+    THEN SUBGOAL_THEN (Term`[~a; &1] poly_divides (r * s)`) MP_TAC
     THENL [
       ALL_TAC,
       ASM_REWRITE_TAC[POLY_PRIMES]
     ]
     THEN REWRITE_TAC[poly_divides]
-    THEN EXISTS_TAC ``t:real list``
-    THEN SUBGOAL_THEN ``poly ([~ a; &1] pexp (poly_order a p) ** (r ** s)) =
-      poly ([~ a; &1] pexp (poly_order a p) ** ([~ a; &1] ** t))`` MP_TAC
+    THEN EXISTS_TAC (Term`t:real list`)
+    THEN SUBGOAL_THEN (Term`poly ([~ a; &1] poly_exp (poly_order a p) * (r * s)) =
+      poly ([~ a; &1] poly_exp (poly_order a p) * ([~ a; &1] * t))`) MP_TAC
     THENL [
       ALL_TAC,
       MESON_TAC[POLY_MUL_LCANCEL, POLY_EXP_PRIME_EQ_0]
     ]
-    THEN SUBGOAL_THEN ``poly ([~ a; &1] pexp (poly_order a q) **
-                        ([~ a; &1] pexp (poly_order a p) ** (r ** s))) =
-                  poly ([~ a; &1] pexp (poly_order a q) **
-                        ([~ a; &1] pexp (poly_order a p) **
-                         ([~ a; &1] ** t)))`` MP_TAC
+    THEN SUBGOAL_THEN (Term`poly ([~ a; &1] poly_exp (poly_order a q) *
+                        ([~ a; &1] poly_exp (poly_order a p) * (r * s))) =
+                  poly ([~ a; &1] poly_exp (poly_order a q) *
+                        ([~ a; &1] poly_exp (poly_order a p) *
+                         ([~ a; &1] * t)))`) MP_TAC
     THENL [
       ALL_TAC,
       MESON_TAC[POLY_MUL_LCANCEL, POLY_EXP_PRIME_EQ_0]
@@ -1084,51 +1106,51 @@ val ORDER_MUL = store_thm("ORDER_MUL",
   ]);
 
 val ORDER_DIFF = store_thm("ORDER_DIFF",
- ``!p a. ~(poly (diff p) = poly []) /\
+ (Term`!p a. ~(poly (diff p) = poly []) /\
          ~(poly_order a p = 0)
-         ==> (poly_order a p = SUC (poly_order a (diff p)))``,
+         ==> (poly_order a p = SUC (poly_order a (diff p)))`),
   REPEAT GEN_TAC THEN
   DISCH_THEN(CONJUNCTS_THEN2 ASSUME_TAC MP_TAC) THEN
-  SUBGOAL_THEN ``~(poly p = poly [])`` MP_TAC THENL
+  SUBGOAL_THEN (Term`~(poly p = poly [])`) MP_TAC THENL
    [ASM_MESON_TAC[POLY_DIFF_ZERO], ALL_TAC] THEN
-  DISCH_THEN(X_CHOOSE_THEN ``q:real list`` MP_TAC o
-    SPEC ``a:real`` o MATCH_MP ORDER_DECOMP) THEN
-  SPEC_TAC(``poly_order a p``,``n:num``) THEN
+  DISCH_THEN(X_CHOOSE_THEN (Term`q:real list`) MP_TAC o
+    SPEC (Term`a:real`) o MATCH_MP ORDER_DECOMP) THEN
+  SPEC_TAC((Term`poly_order a p`),(Term`n:num`)) THEN
   INDUCT_TAC THEN REWRITE_TAC[NOT_SUC, SUC_INJ] THEN
   STRIP_TAC THEN MATCH_MP_TAC ORDER_UNIQUE THEN
   ASM_REWRITE_TAC[] THEN
-  SUBGOAL_THEN ``!r. r poly_divides (diff p) =
-                    r poly_divides (diff ([~ a; &1] pexp SUC n ** q))``
+  SUBGOAL_THEN (Term`!r. r poly_divides (diff p) =
+                    r poly_divides (diff ([~ a; &1] poly_exp SUC n * q))`)
   (fn th => REWRITE_TAC[th]) THENL
    [GEN_TAC THEN REWRITE_TAC[poly_divides] THEN
     FIRST_ASSUM(fn th => REWRITE_TAC[MATCH_MP POLY_DIFF_WELLDEF th]),
     ALL_TAC] THEN
   CONJ_TAC THENL
    [REWRITE_TAC[poly_divides, FUN_EQ_THM] THEN
-    EXISTS_TAC ``[~a; &1] ** (diff q) ++ &(SUC n) ## q`` THEN
+    EXISTS_TAC (Term`[~a; &1] * (diff q) + &(SUC n) ## q`) THEN
     REWRITE_TAC[POLY_DIFF_MUL, POLY_DIFF_EXP_PRIME,
       POLY_ADD, POLY_MUL, POLY_CMUL] THEN
-    REWRITE_TAC[poly_pexp, POLY_MUL] THEN REAL_ARITH_TAC,
+    REWRITE_TAC[poly_exp, POLY_MUL] THEN REAL_ARITH_TAC,
     REWRITE_TAC[FUN_EQ_THM, poly_divides, POLY_DIFF_MUL, POLY_DIFF_EXP_PRIME,
       POLY_ADD, POLY_MUL, POLY_CMUL] THEN
-    DISCH_THEN(X_CHOOSE_THEN ``r:real list`` ASSUME_TAC) THEN
-    UNDISCH_TAC ``~([~ a; &1] poly_divides q)`` THEN
+    DISCH_THEN(X_CHOOSE_THEN (Term`r:real list`) ASSUME_TAC) THEN
+    UNDISCH_TAC (Term`~([~ a; &1] poly_divides q)`) THEN
     REWRITE_TAC[poly_divides] THEN
-    EXISTS_TAC ``inv(&(SUC n)) ## (r ++ neg(diff q))`` THEN
+    EXISTS_TAC (Term`inv(&(SUC n)) ## (r + poly_neg(diff q))`) THEN
     SUBGOAL_THEN
-        ``poly ([~a; &1] pexp n ** q) =
-         poly ([~a; &1] pexp n ** ([~ a; &1] ** (inv (&(SUC n)) ##
-                                   (r ++ neg (diff q)))))``
+        (Term`poly ([~a; &1] poly_exp n * q) =
+         poly ([~a; &1] poly_exp n * ([~ a; &1] * (inv (&(SUC n)) ##
+                                   (r + poly_neg (diff q)))))`)
     MP_TAC THENL
      [ALL_TAC, MESON_TAC[POLY_MUL_LCANCEL, POLY_EXP_PRIME_EQ_0]] THEN
-    REWRITE_TAC[FUN_EQ_THM] THEN X_GEN_TAC ``x:real`` THEN
+    REWRITE_TAC[FUN_EQ_THM] THEN X_GEN_TAC (Term`x:real`) THEN
     SUBGOAL_THEN
-        ``!a b. (&(SUC n) * a = &(SUC n) * b) ==> (a = b)``
+        (Term`!a b. (&(SUC n) * a = &(SUC n) * b) ==> (a = b)`)
     MATCH_MP_TAC THENL
      [REWRITE_TAC[REAL_EQ_MUL_LCANCEL, REAL_OF_NUM_EQ, NOT_SUC], ALL_TAC] THEN
     REWRITE_TAC[POLY_MUL, POLY_CMUL] THEN
-    SUBGOAL_THEN ``!a b c. &(SUC n) * (a * (b * (inv(&(SUC n)) * c))) =
-                          a * (b * c)``
+    SUBGOAL_THEN (Term`!a b c. &(SUC n) * (a * (b * (inv(&(SUC n)) * c))) =
+                          a * (b * c)`)
     (fn th => REWRITE_TAC[th]) THENL
       [REPEAT GEN_TAC THEN
        GEN_REWRITE_TAC LAND_CONV [REAL_MUL_SYM] THEN
@@ -1139,8 +1161,8 @@ val ORDER_DIFF = store_thm("ORDER_DIFF",
        REWRITE_TAC[GSYM REAL_MUL_ASSOC] THEN AP_TERM_TAC THEN
        MATCH_MP_TAC REAL_MUL_RINV THEN
        REWRITE_TAC[REAL_OF_NUM_EQ, NOT_SUC], ALL_TAC] THEN
-    FIRST_ASSUM(MP_TAC o SPEC ``x:real``) THEN
-    REWRITE_TAC[poly_pexp, POLY_MUL, POLY_ADD, POLY_NEG] THEN
+    FIRST_ASSUM(MP_TAC o SPEC (Term`x:real`)) THEN
+    REWRITE_TAC[poly_exp, POLY_MUL, POLY_ADD, POLY_NEG] THEN
     REAL_ARITH_TAC]);
 
 (* ------------------------------------------------------------------------- *)
@@ -1148,51 +1170,51 @@ val ORDER_DIFF = store_thm("ORDER_DIFF",
 (* ------------------------------------------------------------------------- *)
 
 val POLY_SQUAREFREE_DECOMP_ORDER = store_thm("POLY_SQUAREFREE_DECOMP_ORDER",
- ``!p q d e r s.
+ (Term`!p q d e r s.
         ~(poly (diff p) = poly []) /\
-        (poly p = poly (q ** d)) /\
-        (poly (diff p) = poly (e ** d)) /\
-        (poly d = poly (r ** p ++ s ** diff p))
-        ==> !a. poly_order a q = (if (poly_order a p = 0) then 0 else 1)``,
+        (poly p = poly (q * d)) /\
+        (poly (diff p) = poly (e * d)) /\
+        (poly d = poly (r * p + s * diff p))
+        ==> !a. poly_order a q = (if (poly_order a p = 0) then 0 else 1)`),
   REPEAT STRIP_TAC THEN
-  SUBGOAL_THEN ``poly_order a p = poly_order a q + poly_order a d`` MP_TAC THENL
-   [MATCH_MP_TAC EQ_TRANS THEN EXISTS_TAC ``poly_order a (q ** d)`` THEN
+  SUBGOAL_THEN (Term`poly_order a p = poly_order a q + poly_order a d`) MP_TAC THENL
+   [MATCH_MP_TAC EQ_TRANS THEN EXISTS_TAC (Term`poly_order a (q * d)`) THEN
     CONJ_TAC THENL
      [MATCH_MP_TAC ORDER_POLY THEN ASM_REWRITE_TAC[],
       MATCH_MP_TAC ORDER_MUL THEN
       FIRST_ASSUM(fn th =>
         GEN_REWRITE_TAC (RAND_CONV o LAND_CONV) [SYM th]) THEN
       ASM_MESON_TAC[POLY_DIFF_ZERO]], ALL_TAC] THEN
-  ASM_CASES_TAC ``poly_order a p = 0`` THEN ASM_REWRITE_TAC[] THENL
+  ASM_CASES_TAC (Term`poly_order a p = 0`) THEN ASM_REWRITE_TAC[] THENL
    [ARITH_TAC, ALL_TAC] THEN
-  SUBGOAL_THEN ``poly_order a (diff p) =
-                poly_order a e + poly_order a d`` MP_TAC THENL
-   [MATCH_MP_TAC EQ_TRANS THEN EXISTS_TAC ``poly_order a (e ** d)`` THEN
+  SUBGOAL_THEN (Term`poly_order a (diff p) =
+                poly_order a e + poly_order a d`) MP_TAC THENL
+   [MATCH_MP_TAC EQ_TRANS THEN EXISTS_TAC (Term`poly_order a (e * d)`) THEN
     CONJ_TAC THENL
      [ASM_MESON_TAC[ORDER_POLY], ASM_MESON_TAC[ORDER_MUL]], ALL_TAC] THEN
-  SUBGOAL_THEN ``~(poly p = poly [])`` ASSUME_TAC THENL
+  SUBGOAL_THEN (Term`~(poly p = poly [])`) ASSUME_TAC THENL
    [ASM_MESON_TAC[POLY_DIFF_ZERO], ALL_TAC] THEN
-  MP_TAC(SPECL [``p:real list``, ``a:real``] ORDER_DIFF) THEN
+  MP_TAC(SPECL [(Term`p:real list`), (Term`a:real`)] ORDER_DIFF) THEN
   ASM_REWRITE_TAC[] THEN
-  DISCH_THEN(fn th => MP_TAC th THEN MP_TAC(AP_TERM ``PRE`` th)) THEN
+  DISCH_THEN(fn th => MP_TAC th THEN MP_TAC(AP_TERM (Term`PRE`) th)) THEN
   REWRITE_TAC[PRE] THEN DISCH_THEN(ASSUME_TAC o SYM) THEN
-  SUBGOAL_THEN ``poly_order a (diff p) <= poly_order a d`` MP_TAC THENL
-   [SUBGOAL_THEN ``([~a; &1] pexp (poly_order a (diff p))) poly_divides d``
+  SUBGOAL_THEN (Term`poly_order a (diff p) <= poly_order a d`) MP_TAC THENL
+   [SUBGOAL_THEN (Term`([~a; &1] poly_exp (poly_order a (diff p))) poly_divides d`)
     MP_TAC THENL [ALL_TAC, ASM_MESON_TAC[POLY_ENTIRE, ORDER_DIVIDES]] THEN
     SUBGOAL_THEN
-      ``([~a; &1] pexp (poly_order a (diff p))) poly_divides p /\
-       ([~a; &1] pexp (poly_order a (diff p))) poly_divides (diff p)``
+      (Term`([~a; &1] poly_exp (poly_order a (diff p))) poly_divides p /\
+       ([~a; &1] poly_exp (poly_order a (diff p))) poly_divides (diff p)`)
     MP_TAC THENL
      [REWRITE_TAC[ORDER_DIVIDES, LE_REFL] THEN DISJ2_TAC THEN
-      REWRITE_TAC[ASSUME ``poly_order a (diff p) = PRE (poly_order a p)``] THEN
+      REWRITE_TAC[ASSUME (Term`poly_order a (diff p) = PRE (poly_order a p)`)] THEN
       ARITH_TAC,
       DISCH_THEN(CONJUNCTS_THEN MP_TAC) THEN REWRITE_TAC[poly_divides] THEN
-      REWRITE_TAC[ASSUME ``poly d = poly (r ** p ++ s ** diff p)``] THEN
+      REWRITE_TAC[ASSUME (Term`poly d = poly (r * p + s * diff p)`)] THEN
       POP_ASSUM_LIST(K ALL_TAC) THEN
       SIMP_TAC bool_ss [FUN_EQ_THM, POLY_MUL, POLY_ADD] THEN
-      DISCH_THEN(X_CHOOSE_THEN ``f:real list`` ASSUME_TAC) THEN
-      DISCH_THEN(X_CHOOSE_THEN ``g:real list`` ASSUME_TAC) THEN
-      EXISTS_TAC ``r ** g ++ s ** f``
+      DISCH_THEN(X_CHOOSE_THEN (Term`f:real list`) ASSUME_TAC) THEN
+      DISCH_THEN(X_CHOOSE_THEN (Term`g:real list`) ASSUME_TAC) THEN
+      EXISTS_TAC (Term`r * g + s * f`)
       THEN GEN_TAC
       THEN SIMP_TAC real_ss [POLY_MUL, POLY_ADD, REAL_LDISTRIB]
       THEN ASM_REWRITE_TAC [] THEN REAL_ARITH_TAC],
@@ -1203,78 +1225,78 @@ val POLY_SQUAREFREE_DECOMP_ORDER = store_thm("POLY_SQUAREFREE_DECOMP_ORDER",
 (* ------------------------------------------------------------------------- *)
 
 val rsquarefree = new_definition ("rsquarefree",
-  ``rsquarefree p = ~(poly p = poly []) /\
-                   !a. (poly_order a p = 0) \/ (poly_order a p = 1)``);
+  (Term`rsquarefree p = ~(poly p = poly []) /\
+                   !a. (poly_order a p = 0) \/ (poly_order a p = 1)`));
 
 (* ------------------------------------------------------------------------- *)
 (* Standard squarefree criterion and rephasing of squarefree decomposition.  *)
 (* ------------------------------------------------------------------------- *)
 
 val RSQUAREFREE_ROOTS = store_thm("RSQUAREFREE_ROOTS",
- ``!p. rsquarefree p = !a. ~((poly p a = &0) /\ (poly (diff p) a = &0))``,
+ (Term`!p. rsquarefree p = !a. ~((poly p a = &0) /\ (poly (diff p) a = &0))`),
   GEN_TAC THEN REWRITE_TAC[rsquarefree] THEN
-  ASM_CASES_TAC ``poly p = poly []`` THEN ASM_REWRITE_TAC[] THENL
+  ASM_CASES_TAC (Term`poly p = poly []`) THEN ASM_REWRITE_TAC[] THENL
    [FIRST_ASSUM(SUBST1_TAC o MATCH_MP POLY_DIFF_ZERO) THEN
     ASM_REWRITE_TAC[poly, NOT_FORALL_THM],
-    ASM_CASES_TAC ``poly(diff p) = poly []`` THEN ASM_REWRITE_TAC[] THENL
-     [FIRST_ASSUM(X_CHOOSE_THEN ``h:real`` MP_TAC o
+    ASM_CASES_TAC (Term`poly(diff p) = poly []`) THEN ASM_REWRITE_TAC[] THENL
+     [FIRST_ASSUM(X_CHOOSE_THEN (Term`h:real`) MP_TAC o
         MATCH_MP POLY_DIFF_ISZERO) THEN
       DISCH_THEN(fn th => ASSUME_TAC th THEN MP_TAC th) THEN
       DISCH_THEN(fn th => REWRITE_TAC[MATCH_MP ORDER_POLY th]) THEN
-      UNDISCH_TAC ``~(poly p = poly [])`` THEN ASM_REWRITE_TAC[poly] THEN
+      UNDISCH_TAC (Term`~(poly p = poly [])`) THEN ASM_REWRITE_TAC[poly] THEN
       REWRITE_TAC[FUN_EQ_THM, poly, REAL_MUL_RZERO, REAL_ADD_RID] THEN
       DISCH_TAC THEN ASM_REWRITE_TAC[] THEN
-      X_GEN_TAC ``a:real`` THEN DISJ1_TAC THEN
-      MP_TAC(SPECL [``[h:real]``, ``a:real``] ORDER_ROOT) THEN
+      X_GEN_TAC (Term`a:real`) THEN DISJ1_TAC THEN
+      MP_TAC(SPECL [(Term`[h:real]`), (Term`a:real`)] ORDER_ROOT) THEN
       ASM_REWRITE_TAC[FUN_EQ_THM, poly, REAL_MUL_RZERO, REAL_ADD_RID],
       ASM_REWRITE_TAC[ORDER_ROOT, DE_MORGAN_THM, ONE] THEN
       ASM_MESON_TAC[ORDER_DIFF, SUC_INJ]]]);
 
 val RSQUAREFREE_DECOMP = store_thm("RSQUAREFREE_DECOMP",
- ``!p a. rsquarefree p /\ (poly p a = &0)
-         ==> ?q. (poly p = poly ([~a; &1] ** q)) /\
-                 ~(poly q a = &0)``,
+ (Term`!p a. rsquarefree p /\ (poly p a = &0)
+         ==> ?q. (poly p = poly ([~a; &1] * q)) /\
+                 ~(poly q a = &0)`),
   REPEAT GEN_TAC THEN REWRITE_TAC[rsquarefree] THEN STRIP_TAC THEN
   FIRST_ASSUM(MP_TAC o MATCH_MP ORDER_DECOMP) THEN
-  DISCH_THEN(X_CHOOSE_THEN ``q:real list`` MP_TAC o SPEC ``a:real``) THEN
+  DISCH_THEN(X_CHOOSE_THEN (Term`q:real list`) MP_TAC o SPEC (Term`a:real`)) THEN
   FIRST_ASSUM(MP_TAC o GEN_REWRITE_RULE I [ORDER_ROOT]) THEN
-  FIRST_ASSUM(DISJ_CASES_TAC o SPEC ``a:real``) THEN
+  FIRST_ASSUM(DISJ_CASES_TAC o SPEC (Term`a:real`)) THEN
   ASM_SIMP_TAC real_ss [] THEN
   DISCH_THEN(CONJUNCTS_THEN2 SUBST_ALL_TAC ASSUME_TAC) THEN
-  EXISTS_TAC ``q:real list`` THEN CONJ_TAC THENL
+  EXISTS_TAC (Term`q:real list`) THEN CONJ_TAC THENL
    [REWRITE_TAC[FUN_EQ_THM, POLY_MUL] THEN GEN_TAC THEN
     AP_THM_TAC THEN AP_TERM_TAC THEN
     GEN_REWRITE_TAC (LAND_CONV o LAND_CONV o RAND_CONV) [ONE] THEN
-    REWRITE_TAC[poly_pexp, POLY_MUL] THEN
+    REWRITE_TAC[poly_exp, POLY_MUL] THEN
     REWRITE_TAC[poly] THEN REAL_ARITH_TAC,
-    DISCH_TAC THEN UNDISCH_TAC ``~([~a; &1] poly_divides q)`` THEN
+    DISCH_TAC THEN UNDISCH_TAC (Term`~([~a; &1] poly_divides q)`) THEN
     REWRITE_TAC[poly_divides] THEN
-    UNDISCH_TAC ``poly q a = &0`` THEN
+    UNDISCH_TAC (Term`poly q a = &0`) THEN
     GEN_REWRITE_TAC LAND_CONV [POLY_LINEAR_DIVIDES] THEN
-    ASM_CASES_TAC ``q:real list = []`` THEN ASM_REWRITE_TAC[] THENL
-     [EXISTS_TAC ``[] : real list`` THEN REWRITE_TAC[FUN_EQ_THM] THEN
+    ASM_CASES_TAC (Term`q:real list = []`) THEN ASM_REWRITE_TAC[] THENL
+     [EXISTS_TAC (Term`[] : real list`) THEN REWRITE_TAC[FUN_EQ_THM] THEN
       REWRITE_TAC[POLY_MUL, poly, REAL_MUL_RZERO],
       MESON_TAC[]]]);
 
 val POLY_SQUAREFREE_DECOMP = store_thm("POLY_SQUAREFREE_DECOMP",
- ``!p q d e r s.
+ (Term`!p q d e r s.
         ~(poly (diff p) = poly []) /\
-        (poly p = poly (q ** d)) /\
-        (poly (diff p) = poly (e ** d)) /\
-        (poly d = poly (r ** p ++ s ** diff p))
-        ==> rsquarefree q /\ (!a. (poly q a = &0) = (poly p a = &0))``,
+        (poly p = poly (q * d)) /\
+        (poly (diff p) = poly (e * d)) /\
+        (poly d = poly (r * p + s * diff p))
+        ==> rsquarefree q /\ (!a. (poly q a = &0) = (poly p a = &0))`),
   REPEAT GEN_TAC THEN DISCH_THEN(fn th => MP_TAC th THEN
     ASSUME_TAC(MATCH_MP POLY_SQUAREFREE_DECOMP_ORDER th)) THEN
   DISCH_THEN(CONJUNCTS_THEN2 ASSUME_TAC MP_TAC) THEN
-  SUBGOAL_THEN ``~(poly p = poly [])`` ASSUME_TAC THENL
+  SUBGOAL_THEN (Term`~(poly p = poly [])`) ASSUME_TAC THENL
    [ASM_MESON_TAC[POLY_DIFF_ZERO], ALL_TAC] THEN
   DISCH_THEN(ASSUME_TAC o CONJUNCT1) THEN
-  UNDISCH_TAC ``~(poly p = poly [])`` THEN
+  UNDISCH_TAC (Term`~(poly p = poly [])`) THEN
   DISCH_THEN(fn th => MP_TAC th THEN MP_TAC th) THEN
   DISCH_THEN(fn th => ASM_REWRITE_TAC[] THEN ASSUME_TAC th) THEN
   ASM_REWRITE_TAC[] THEN
   REWRITE_TAC[POLY_ENTIRE, DE_MORGAN_THM] THEN STRIP_TAC THEN
-  UNDISCH_TAC ``poly p = poly (q ** d)`` THEN
+  UNDISCH_TAC (Term`poly p = poly (q * d)`) THEN
   DISCH_THEN(SUBST_ALL_TAC o SYM) THEN
   ASM_REWRITE_TAC[rsquarefree, ORDER_ROOT] THEN
   CONJ_TAC THEN GEN_TAC THEN COND_CASES_TAC THEN ASM_SIMP_TAC real_ss []);
@@ -1284,17 +1306,17 @@ val POLY_SQUAREFREE_DECOMP = store_thm("POLY_SQUAREFREE_DECOMP",
 (* ------------------------------------------------------------------------- *)
 
 val normalize = new_recursive_definition list_Axiom "normalize"
-  ``(normalize [] = []) /\
+  (Term`(normalize [] = []) /\
    (normalize (CONS h t) = (if (normalize t = []) then
                               if (h = &0) then [] else [h]
-                            else CONS h (normalize t)))``;
+                            else CONS h (normalize t)))`);
 
 val POLY_NORMALIZE = store_thm("POLY_NORMALIZE",
- ``!p. poly (normalize p) = poly p``,
+ (Term`!p. poly (normalize p) = poly p`),
   LIST_INDUCT_TAC THEN REWRITE_TAC[normalize, poly] THEN
-  ASM_CASES_TAC ``h = &0`` THEN ASM_REWRITE_TAC[] THEN
+  ASM_CASES_TAC (Term`h = &0`) THEN ASM_REWRITE_TAC[] THEN
   COND_CASES_TAC THEN ASM_REWRITE_TAC[poly, FUN_EQ_THM] THEN
-  UNDISCH_TAC ``poly (normalize t) = poly t`` THEN
+  UNDISCH_TAC (Term`poly (normalize t) = poly t`) THEN
   DISCH_THEN(SUBST1_TAC o SYM) THEN ASM_REWRITE_TAC[poly] THEN
   REWRITE_TAC[REAL_MUL_RZERO, REAL_ADD_LID]);
 
@@ -1303,17 +1325,17 @@ val POLY_NORMALIZE = store_thm("POLY_NORMALIZE",
 (* ------------------------------------------------------------------------- *)
 
 val degree = new_definition ("degree",
-  ``degree p = PRE(LENGTH(normalize p))``);
+  (Term`degree p = PRE(LENGTH(normalize p))`));
 
 val DEGREE_ZERO = store_thm("DEGREE_ZERO",
- ``!p. (poly p = poly []) ==> (degree p = 0)``,
+ (Term`!p. (poly p = poly []) ==> (degree p = 0)`),
   REPEAT STRIP_TAC THEN REWRITE_TAC[degree] THEN
-  SUBGOAL_THEN ``normalize p = []`` SUBST1_TAC THENL
-   [POP_ASSUM MP_TAC THEN SPEC_TAC(``p:real list``,``p:real list``) THEN
+  SUBGOAL_THEN (Term`normalize p = []`) SUBST1_TAC THENL
+   [POP_ASSUM MP_TAC THEN SPEC_TAC((Term`p:real list`),(Term`p:real list`)) THEN
     REWRITE_TAC[POLY_ZERO] THEN
     LIST_INDUCT_TAC THEN REWRITE_TAC[normalize, FORALL] THEN
     STRIP_TAC THEN ASM_REWRITE_TAC[] THEN
-    SUBGOAL_THEN ``normalize t = []`` (fn th => REWRITE_TAC[th]) THEN
+    SUBGOAL_THEN (Term`normalize t = []`) (fn th => REWRITE_TAC[th]) THEN
     FIRST_ASSUM MATCH_MP_TAC THEN ASM_REWRITE_TAC[],
     REWRITE_TAC[LENGTH, PRE]]);
 
@@ -1322,21 +1344,21 @@ val DEGREE_ZERO = store_thm("DEGREE_ZERO",
 (* ------------------------------------------------------------------------- *)
 
 val POLY_ROOTS_FINITE_SET = store_thm("POLY_ROOTS_FINITE_SET",
- ``!p. ~(poly p = poly []) ==> FINITE {x | poly p x = &0}``,
+ (Term`!p. ~(poly p = poly []) ==> FINITE {x | poly p x = &0}`),
   GEN_TAC THEN REWRITE_TAC[POLY_ROOTS_FINITE] THEN
-  DISCH_THEN(X_CHOOSE_THEN ``N:num`` MP_TAC) THEN
-  DISCH_THEN(X_CHOOSE_THEN ``i:num->real`` ASSUME_TAC) THEN
+  DISCH_THEN(X_CHOOSE_THEN (Term`N:num`) MP_TAC) THEN
+  DISCH_THEN(X_CHOOSE_THEN (Term`i:num->real`) ASSUME_TAC) THEN
   MATCH_MP_TAC FINITE_SUBSET THEN
-  EXISTS_TAC ``{x:real | ?n:num. n < N /\ (x = i n)}`` THEN
+  EXISTS_TAC (Term`{x:real | ?n:num. n < N /\ (x = i n)}`) THEN
   CONJ_TAC THENL
-   [SPEC_TAC(``N:num``,``N:num``) THEN POP_ASSUM_LIST(K ALL_TAC) THEN
+   [SPEC_TAC((Term`N:num`),(Term`N:num`)) THEN POP_ASSUM_LIST(K ALL_TAC) THEN
     INDUCT_TAC THENL
-     [SUBGOAL_THEN ``{x:real | ?n:num. n < 0 /\ (x = i n)} = {}``
+     [SUBGOAL_THEN (Term`{x:real | ?n:num. n < 0 /\ (x = i n)} = {}`)
       (fn th => REWRITE_TAC[th, FINITE_RULES]) THEN
       SIMP_TAC bool_ss [GSPEC_DEF, EMPTY_DEF, pairTheory.CLOSED_PAIR_EQ,
-        NOT_LESS, EQT_ELIM (ARITH_CONV ``!n:num. ~(n < 0)``)],
-      SUBGOAL_THEN ``{x:real | ?n. n < SUC N /\ (x = i n)} =
-                    (i N) INSERT {x:real | ?n:num. n < N /\ (x = i n)}``
+        NOT_LESS, EQT_ELIM (ARITH_CONV (Term`!n:num. ~(n < 0)`))],
+      SUBGOAL_THEN (Term`{x:real | ?n. n < SUC N /\ (x = i n)} =
+                    (i N) INSERT {x:real | ?n:num. n < N /\ (x = i n)}`)
       SUBST1_TAC THENL
        [SIMP_TAC bool_ss [LT, EXTENSION, IN_INSERT, SPECIFICATION,
                           GSPEC_DEF,pairTheory.CLOSED_PAIR_EQ]
@@ -1351,12 +1373,12 @@ val POLY_ROOTS_FINITE_SET = store_thm("POLY_ROOTS_FINITE_SET",
 (* ------------------------------------------------------------------------- *)
 
 val POLY_MONO = store_thm("POLY_MONO",
- ``!x k p. abs(x) <= k ==> abs(poly p x) <= poly (MAP abs p) k``,
+ (Term`!x k p. abs(x) <= k ==> abs(poly p x) <= poly (MAP abs p) k`),
   GEN_TAC THEN GEN_TAC THEN REWRITE_TAC[RIGHT_FORALL_IMP_THM] THEN
   DISCH_TAC THEN LIST_INDUCT_TAC THEN
   REWRITE_TAC[poly, REAL_LE_REFL, MAP, REAL_ABS_0] THEN
   MATCH_MP_TAC REAL_LE_TRANS THEN
-  EXISTS_TAC ``abs(h) + abs(x * poly t x)`` THEN
+  EXISTS_TAC (Term`abs(h) + abs(x * poly t x)`) THEN
   REWRITE_TAC[REAL_ABS_TRIANGLE, REAL_LE_LADD] THEN
   REWRITE_TAC[REAL_ABS_MUL] THEN
   MATCH_MP_TAC REAL_LE_MUL2 THEN ASM_REWRITE_TAC[REAL_ABS_POS]);
@@ -1416,8 +1438,8 @@ val POLY_MUL_CONV =
 
 val POLY_NORMALIZE_CONV =
   let pth = prove
-   (``normalize (CONS h t) =
-      (\n. (n = []) => (h = &0) => [] | [h] | CONS h n) (normalize t)``,
+   ((Term`normalize (CONS h t) =
+      (\n. (n = []) => (h = &0) => [] | [h] | CONS h n) (normalize t)`),
     REWRITE_TAC[normalize]) in
   let norm_conv0 = GEN_REWRITE_CONV I [CONJUNCT1 normalize]
   and norm_conv1 = GEN_REWRITE_CONV I [pth]
